Cleaning including renaming modules and types

ntor/Metareduction_ntor.ec
@@ -3,9 +3,9 @@ require import AllCore FSet FMap Distr DProd List SplitRO FelTactic.
 
 require NTOR_nosid.
 clone import NTOR_nosid as NTOR_mod.
-import NTORc GAKE_mod GAKEc HROc HRO_mod_c DH.G DH.GP DH.FD DH.GP.ZModE.
+import NTORc UAKE_mod UAKEc HROc HRO_mod_c DH.G DH.GP DH.FD DH.GP.ZModE.
 
-module Counter (G : GAKE_nodhs_i) : GAKEc.GAKE_nodhs_i = {
+module Counter (G : UAKE_res_name_i) : UAKEc.UAKE_res_name_i = {
   var ch, cis, cm1, cm2, cm3 : int
 
   include G[c_rev_skey, s_rev_skey, rev_ltkey, c_rev_ephkey, s_rev_ephkey, c_test, s_test]
@@ -57,18 +57,18 @@ op q_h  : { int | 0 <= q_h } as ge0_q_h.
 
 (* ------------------------------------------------------------------------------------------ *)
 (* Introduce stop in original game *)
-module GAKEb_st (S: Server) (C: Client) (H : GAKEc.HROc.RO) : GAKEc.GAKE_nodhs_i = {
+module UAKE_name_st (S: Server) (C: Client) (H : UAKEc.HROc.RO) : UAKEc.UAKE_res_name_i = {
   var b0 : bool 
 
-  var servers : (s_id, GAKEc.server_state) fmap
+  var servers : (s_id, UAKEc.server_state) fmap
   var unreg_ro : (pkey * pkey * s_id * pkey * pkey) fset
   var pk_set : pkey fset
   var x_set : pkey fset
   var y_set : pkey fset
   var stop1, stop2 : bool
 
-  var c_smap: (int, GAKEc.pr_st_client GAKEc.instance_state) fmap
-  var s_smap: (s_id * int, GAKEc.pr_st_server GAKEc.instance_state) fmap
+  var c_smap: (int, UAKEc.c_state UAKEc.instance_state) fmap
+  var s_smap: (s_id * int, UAKEc.s_state UAKEc.instance_state) fmap
   
   var tested: int option
 
@@ -111,7 +111,7 @@ module GAKEb_st (S: Server) (C: Client) (H : GAKEc.HROc.RO) : GAKEc.GAKE_nodhs_i
       kp <@ S(H).keygen();
       stop1 <- stop1 \/ kp.`1 \in pk_set;
       pk_set <- pk_set `|` fset1 kp.`1;
-      servers.[b] <- GAKEc.Honest kp;
+      servers.[b] <- UAKEc.Honest kp;
     }
     return omap get_pkey servers.[b];
   }
@@ -146,7 +146,7 @@ module GAKEb_st (S: Server) (C: Client) (H : GAKEc.HROc.RO) : GAKEc.GAKE_nodhs_i
     var sko, resp, st', k, m3;
     var r <- None;
 
-    sko <- obind GAKEc.get_skey servers.[b];
+    sko <- obind UAKEc.get_skey servers.[b];
 
     if (sko is Some sk) (* Server was initialised as honest *) {
       match s_smap.[b, j] with
@@ -315,7 +315,7 @@ module GAKEb_st (S: Server) (C: Client) (H : GAKEc.HROc.RO) : GAKEc.GAKE_nodhs_i
     | Some st => {
         (* only accepted server instances that are not ltkey revealed in case they 
            or all partners are tested can be ephkey revealed *)
-        if (st is GAKEc.Accepted st t k ir) { (* No Pending on Server side *)
+        if (st is UAKEc.Accepted st t k ir) { (* No Pending on Server side *)
           if (!((   get_ir_test (oget s_smap.[b, j])
                  \/ untested_partner_s t c_smap = Some false)
                 /\ get_sr_ltk (oget servers.[b]))) {
@@ -392,23 +392,21 @@ module GAKEb_st (S: Server) (C: Client) (H : GAKEc.HROc.RO) : GAKEc.GAKE_nodhs_i
   }
 }.
 
-
 (* ------------------------------------------------------------------------------------------ *)
-(* Reduction from restricted to non-restricted model  *)
-module (Dh_Red (A : GAKEc.A_GAKE_nodhs) : GAKEc.A_GAKE) (O : GAKEc.GAKE) = {
-  module O_GAKE : GAKEc.GAKE_nodhs = {
+(* Reduction from restricted to non-restricted model in the name-based setting *)
+module (Res_Red (A : UAKEc.A_UAKE_res_name) : UAKEc.A_UAKE_unres_name) (O : UAKEc.UAKE_unres_name) = {
+  module O_UAKE_RN : UAKEc.UAKE_res_name = {
    include O [-set_cert]
   }
 
   proc run() : bool = {
     var b';
 
-    b' <@ A(O_GAKE).run();
+    b' <@ A(O_UAKE_RN).run();
 
     return b';
   }
 }.
-
 
 (* ------------------------------------------------------------------------------------------ *)
 (* Reduction to honest game that only allows clients to interact with honest servers  *)
@@ -429,11 +427,11 @@ op get_sr_in s_st : bool =
 with s_st = Inner _ bool => bool
 with s_st = Outer _ => true.
 
-module (Hon_Red (A : GAKEc.A_GAKE) : GAKEc.A_GAKE) (O : GAKEc.GAKE) = {
-  module O_GAKE : GAKEc.GAKE = {
+module (Hon_Red (A : UAKEc.A_UAKE_unres_name) : UAKEc.A_UAKE_unres_name) (O : UAKEc.UAKE_unres_name) = {
+  module O_UAKE_HN : UAKEc.UAKE_unres_name = {
     var dh_ro : (pkey * pkey * s_id * pkey * pkey, (tag * key)) fmap
     var c_inst : (int, bool) fmap
-    var dhc_smap : (int, GAKEc.pr_st_client GAKEc.instance_state) fmap
+    var dhc_smap : (int, UAKEc.c_state UAKEc.instance_state) fmap
     var servers : (s_id, server_state_mod) fmap
 
     proc h = O.h
@@ -476,7 +474,7 @@ module (Hon_Red (A : GAKEc.A_GAKE) : GAKEc.A_GAKE) (O : GAKEc.GAKE) = {
             pk_ce <- g ^ sk_ce;
             pk_b <- get_pkey_mod (oget servers.[m1]);
             r <- Some pk_ce;
-            dhc_smap.[i] <- GAKEc.Pending (m1, pk_b, sk_ce) (m1, pk_ce) (false, false, false, false);
+            dhc_smap.[i] <- UAKEc.Pending (m1, pk_b, sk_ce) (m1, pk_ce) (false, false, false, false);
             c_inst.[i] <- true;
           }
         }
@@ -498,22 +496,22 @@ module (Hon_Red (A : GAKEc.A_GAKE) : GAKEc.A_GAKE) (O : GAKEc.GAKE) = {
         | None => { } (* Abort? *)
         | Some st => {
             match st with
-            | GAKEc.Pending st pt ir => {
+            | UAKEc.Pending st pt ir => {
                 (b, pk_b, sk_ce) <- st;
                 (t_A, k) <@ O.h(m3.`1 ^ sk_ce, pk_b ^ sk_ce, b, g ^ sk_ce, m3.`1);
                 if (t_A = m3.`2) {
                   if (get_sr_in (oget servers.[pt.`1])) {
-                    dhc_smap.[i] <- set_ir_cor (GAKEc.Accepted st (pt, Some m3) k ir);
+                    dhc_smap.[i] <- set_ir_cor (UAKEc.Accepted st (pt, Some m3) k ir);
                   } else {
-                    dhc_smap.[i] <- GAKEc.Accepted st (pt, Some m3) k ir;
+                    dhc_smap.[i] <- UAKEc.Accepted st (pt, Some m3) k ir;
                   }
                   r <- Some ();
                 } else {
-                  dhc_smap.[i] <- GAKEc.Aborted (Some st) (Some (pt, Some m3)) ir;
+                  dhc_smap.[i] <- UAKEc.Aborted (Some st) (Some (pt, Some m3)) ir;
                 }
               }
-            | GAKEc.Accepted _ _ _ _ => { }
-            | GAKEc.Aborted _ _ _ => { }
+            | UAKEc.Accepted _ _ _ _ => { }
+            | UAKEc.Aborted _ _ _ => { }
             end;
           }
         end;
@@ -531,14 +529,14 @@ module (Hon_Red (A : GAKEc.A_GAKE) : GAKEc.A_GAKE) (O : GAKEc.GAKE) = {
         | None => { }
         | Some st => {
             match st with 
-            | GAKEc.Pending _ _ _ => { }
-            | GAKEc.Accepted st' t' k' ir' => {
+            | UAKEc.Pending _ _ _ => { }
+            | UAKEc.Accepted st' t' k' ir' => {
                 if (!get_ir_test (oget dhc_smap.[i])) { (* removed check on the partner and that they are untested, since an unhonest servers cannot be tested *)
                   r <- Some k';
-                  dhc_smap.[i] <- set_ir_sess (GAKEc.Accepted st' t' k' ir');
+                  dhc_smap.[i] <- set_ir_sess (UAKEc.Accepted st' t' k' ir');
                 }
               }
-            | GAKEc.Aborted _ _ _ => { }
+            | UAKEc.Aborted _ _ _ => { }
             end;
           }
         end;
@@ -576,17 +574,17 @@ module (Hon_Red (A : GAKEc.A_GAKE) : GAKEc.A_GAKE) (O : GAKEc.GAKE) = {
         | None => { }
         | Some st => {
             match st with
-            | GAKEc.Pending st pk_e ir => {
+            | UAKEc.Pending st pk_e ir => {
                 r <- Some (st.`3);
-                dhc_smap.[i] <- set_ir_eph (GAKEc.Pending st pk_e ir);
+                dhc_smap.[i] <- set_ir_eph (UAKEc.Pending st pk_e ir);
               }
-            | GAKEc.Accepted st t k ir => {
+            | UAKEc.Accepted st t k ir => {
                 if (!get_ir_test (oget dhc_smap.[i])) {
                   r <- Some (st.`3);
-                  dhc_smap.[i] <- set_ir_eph (GAKEc.Accepted st t k ir);
+                  dhc_smap.[i] <- set_ir_eph (UAKEc.Accepted st t k ir);
                 }
               }
-            | GAKEc.Aborted _ _ _ => {  }
+            | UAKEc.Aborted _ _ _ => {  }
              end;
           }
         end;
@@ -630,19 +628,19 @@ module (Hon_Red (A : GAKEc.A_GAKE) : GAKEc.A_GAKE) (O : GAKEc.GAKE) = {
   proc run() : bool = {
     var b';
 
-    O_GAKE.dhc_smap <- empty;
-    O_GAKE.c_inst <- empty;
-    O_GAKE.dh_ro <- empty;
-    O_GAKE.servers <- empty;
+    O_UAKE_HN.dhc_smap <- empty;
+    O_UAKE_HN.c_inst <- empty;
+    O_UAKE_HN.dh_ro <- empty;
+    O_UAKE_HN.servers <- empty;
 
-    b' <@ A(O_GAKE).run();
+    b' <@ A(O_UAKE_HN).run();
 
     return b';
   }
 }.
 
-module (Hon_s_Red (A : GAKEc.A_GAKE) : GAKEc.A_GAKE_nodhs) (O : GAKEc.GAKE_nodhs) = {
-  module O_GAKE : GAKEc.GAKE = {
+module (Hon_s_Red (A : UAKEc.A_UAKE_unres_name) : UAKEc.A_UAKE_res_name) (O : UAKEc.UAKE_res_name) = {
+  module O_UAKE : UAKEc.UAKE_unres_name = {
     var servers : (s_id, (bool * pkey option)) fmap
 
     include O [-init_s]
@@ -673,9 +671,9 @@ module (Hon_s_Red (A : GAKEc.A_GAKE) : GAKEc.A_GAKE_nodhs) (O : GAKEc.GAKE_nodhs
   proc run() : bool = {
     var b';
 
-    O_GAKE.servers <- empty;
+    O_UAKE.servers <- empty;
 
-    b' <@ A(O_GAKE).run();
+    b' <@ A(O_UAKE).run();
 
     return b';
   }
@@ -685,8 +683,8 @@ module (Hon_s_Red (A : GAKEc.A_GAKE) : GAKEc.A_GAKE_nodhs) (O : GAKEc.GAKE_nodhs
 (* ------------------------------------------------------------------------------------------ *)
 (* Reduction preventing collisions and prediction of public keys  *)
 
-module (Name_Red (A : GAKEc.A_GAKE_nodhs) : GAKE_mod.A_GAKE_nodhs) (O : GAKE_mod.GAKE_nodhs) = {
-  module O_GAKE : GAKEc.GAKE_nodhs = {
+module (Name_Red (A : UAKEc.A_UAKE_res_name) : UAKE_mod.A_UAKE_res_pk) (O : UAKE_mod.UAKE_res_pk) = {
+  module O_UAKE_RN : UAKEc.UAKE_res_name = {
     var unreg_ro : (pkey * pkey * s_id * pkey * pkey, (tag * key)) fmap
 
     var sid_pk : (s_id, pkey) fmap
@@ -697,7 +695,7 @@ module (Name_Red (A : GAKEc.A_GAKE_nodhs) : GAKE_mod.A_GAKE_nodhs) (O : GAKE_mod
     var stop1 : bool
     var stop2 : bool
 
-    proc h(x : GAKEc.h_input) = {
+    proc h(x : UAKEc.h_input) = {
       var pk_s, tk;
       var r <- (witness, witness);
 
@@ -870,20 +868,19 @@ module (Name_Red (A : GAKEc.A_GAKE_nodhs) : GAKE_mod.A_GAKE_nodhs) (O : GAKE_mod
   proc run() : bool = {
     var b';
 
-    O_GAKE.unreg_ro <- empty;
-    O_GAKE.sid_pk <- empty;
-    O_GAKE.pk_set <- fset0;
-    O_GAKE.x_set <- fset0;
-    O_GAKE.y_set <- fset0;
-    O_GAKE.stop1 <- false;
-    O_GAKE.stop2 <- false;
+    O_UAKE_RN.unreg_ro <- empty;
+    O_UAKE_RN.sid_pk <- empty;
+    O_UAKE_RN.pk_set <- fset0;
+    O_UAKE_RN.x_set <- fset0;
+    O_UAKE_RN.y_set <- fset0;
+    O_UAKE_RN.stop1 <- false;
+    O_UAKE_RN.stop2 <- false;
 
-    b' <@ A(O_GAKE).run();
+    b' <@ A(O_UAKE_RN).run();
 
     return b';
   }
 }.
-
 
 
 (* ------------------------------------------------------------------------------------------ *)
@@ -891,11 +888,11 @@ module (Name_Red (A : GAKEc.A_GAKE_nodhs) : GAKE_mod.A_GAKE_nodhs) (O : GAKE_mod
 (* ------------------------------------------------------------------------------------------ *)
 section.
 
-declare module A <: GAKEc.A_GAKE {-GAKE_mod.HROc.RO, -GAKEc.HROc.RO, -Hon_Red, -Hon_s_Red, -Name_Red, -GAKEc.GAKEb, -GAKEc.GAKEb_hon, -GAKEc.GAKEb_nodhs, -GAKEb_st, -GAKE_mod.GAKEb_nodhs, -Counter }.
+declare module A <: UAKEc.A_UAKE_unres_name {-UAKE_mod.HROc.RO, -UAKEc.HROc.RO, -Hon_Red, -Hon_s_Red, -Name_Red, -UAKEc.O_UN, -UAKEc.O_HN, -UAKEc.O_RN, -UAKE_name_st, -UAKE_mod.O_RPK, -Counter }.
 
-declare module A_res <: GAKEc.A_GAKE_nodhs {-GAKE_mod.HROc.RO, -GAKEc.HROc.RO, -Hon_Red, -Hon_s_Red, -Name_Red, -GAKEc.GAKEb, -GAKEc.GAKEb_hon, -GAKEc.GAKEb_nodhs, -GAKEb_st, -GAKE_mod.GAKEb_nodhs, -Counter }.
+declare module A_res <: UAKEc.A_UAKE_res_name {-UAKE_mod.HROc.RO, -UAKEc.HROc.RO, -Hon_Red, -Hon_s_Red, -Name_Red, -UAKEc.O_UN, -UAKEc.O_HN, -UAKEc.O_RN, -UAKE_name_st, -UAKE_mod.O_RPK, -Counter }.
 
-declare axiom A_ll (G <: GAKEc.GAKE{-A}):
+declare axiom A_ll (G <: UAKEc.UAKE_unres_name{-A}):
   islossless G.h =>
   islossless G.init_s =>
   islossless G.set_cert =>
@@ -911,7 +908,7 @@ declare axiom A_ll (G <: GAKEc.GAKE{-A}):
   islossless G.s_test => 
   islossless A(G).run. 
 
-declare axiom B_ll (G <: GAKEc.GAKE_nodhs{-A_res}):
+declare axiom B_ll (G <: UAKEc.UAKE_res_name{-A_res}):
   islossless G.h =>
   islossless G.init_s =>
   islossless G.send_msg1 =>
@@ -926,46 +923,44 @@ declare axiom B_ll (G <: GAKEc.GAKE_nodhs{-A_res}):
   islossless G.s_test => 
   islossless A_res(G).run.
 
-declare axiom A_res_bounded_qs: forall (G <: GAKEc.GAKE_nodhs_i{-A_res}), hoare[A_res(Counter(G)).run: Counter.cis = 0 /\ Counter.cm1 = 0 /\ Counter.cm2 = 0 /\ Counter.cm3 = 0 /\ Counter.ch = 0
+declare axiom A_res_bounded_qs: forall (G <: UAKEc.UAKE_res_name_i{-A_res}), hoare[A_res(Counter(G)).run: Counter.cis = 0 /\ Counter.cm1 = 0 /\ Counter.cm2 = 0 /\ Counter.cm3 = 0 /\ Counter.ch = 0
                                                                   ==> Counter.cis < q_is /\ Counter.cm1 < q_m1 /\ Counter.cm2 < q_m2 /\ Counter.cm3 < q_m3 /\ Counter.ch < q_h].
  
-
 local lemma fset0_nin (s : 'a fset) x : s = fset0 => x \notin s.
 proof.
 move => ->.
 by rewrite in_fset0.
 qed.
 
-
-lemma sum_stop bit &m: Pr[GAKEc.E_GAKE_nodhs(GAKEb_st(NTOR_S, NTOR_C, GAKEc.HROc.RO), A_res).run(bit) @ &m : (GAKEb_st.stop1 \/ GAKEb_st.stop2)] 
-  <= Pr[GAKEc.E_GAKE_nodhs(GAKEb_st(NTOR_S, NTOR_C, GAKEc.HROc.RO), A_res).run(bit) @ &m : GAKEb_st.stop1] 
-      + Pr[GAKEc.E_GAKE_nodhs(GAKEb_st(NTOR_S, NTOR_C, GAKEc.HROc.RO), A_res).run(bit) @ &m : GAKEb_st.stop2].
+lemma sum_stop bit &m: Pr[UAKEc.E_UAKE_RN(UAKE_name_st(NTOR_S, NTOR_C, UAKEc.HROc.RO), A_res).run(bit) @ &m : (UAKE_name_st.stop1 \/ UAKE_name_st.stop2)] 
+  <= Pr[UAKEc.E_UAKE_RN(UAKE_name_st(NTOR_S, NTOR_C, UAKEc.HROc.RO), A_res).run(bit) @ &m : UAKE_name_st.stop1] 
+      + Pr[UAKEc.E_UAKE_RN(UAKE_name_st(NTOR_S, NTOR_C, UAKEc.HROc.RO), A_res).run(bit) @ &m : UAKE_name_st.stop2].
 proof.
 rewrite Pr[mu_or].
 smt(ge0_mu).
 qed.
 
-lemma bound_stop1 bit &m: Pr[GAKEc.E_GAKE_nodhs(GAKEb_st(NTOR_S, NTOR_C, GAKEc.HROc.RO), A_res).run(bit) @ &m : GAKEb_st.stop1] 
+lemma bound_stop1 bit &m: Pr[UAKEc.E_UAKE_RN(UAKE_name_st(NTOR_S, NTOR_C, UAKEc.HROc.RO), A_res).run(bit) @ &m : UAKE_name_st.stop1] 
   <= ((q_is + q_m1 + q_m2) * (q_is + q_m1 + q_m2 - 1))%r / (2 * order)%r.
 proof.
-have ->: Pr[E_GAKE_nodhs(GAKEb_st(NTOR_S, NTOR_C, GAKEc.HROc.RO), A_res).run(bit) @ &m : GAKEb_st.stop1]
-       = Pr[E_GAKE_nodhs(Counter(GAKEb_st(NTOR_S, NTOR_C, GAKEc.HROc.RO)), A_res).run(bit) @ &m : GAKEb_st.stop1].
+have ->: Pr[E_UAKE_RN(UAKE_name_st(NTOR_S, NTOR_C, UAKEc.HROc.RO), A_res).run(bit) @ &m : UAKE_name_st.stop1]
+       = Pr[E_UAKE_RN(Counter(UAKE_name_st(NTOR_S, NTOR_C, UAKEc.HROc.RO)), A_res).run(bit) @ &m : UAKE_name_st.stop1].
 + byequiv => //.
   proc.
-  call (: ={glob GAKEb_st, glob HROc.RO}); try (proc; inline; sim />).
+  call (: ={glob UAKE_name_st, glob HROc.RO}); try (proc; inline; sim />).
   + proc; inline. 
     by sp; if; auto.
   + by auto => />. 
   + by auto => />. 
   + by auto => />. 
   by inline; auto => />.
-have ->: Pr[E_GAKE_nodhs(Counter(GAKEb_st(NTOR_S, NTOR_C, GAKEc.HROc.RO)), A_res).run(bit) @ &m : GAKEb_st.stop1]
-       = Pr[E_GAKE_nodhs(Counter(GAKEb_st(NTOR_S, NTOR_C, GAKEc.HROc.RO)), A_res).run(bit) @ &m : GAKEb_st.stop1
+have ->: Pr[E_UAKE_RN(Counter(UAKE_name_st(NTOR_S, NTOR_C, UAKEc.HROc.RO)), A_res).run(bit) @ &m : UAKE_name_st.stop1]
+       = Pr[E_UAKE_RN(Counter(UAKE_name_st(NTOR_S, NTOR_C, UAKEc.HROc.RO)), A_res).run(bit) @ &m : UAKE_name_st.stop1
             /\ Counter.cis < q_is /\ Counter.cm1 < q_m1 /\ Counter.cm2 < q_m2].
 + byequiv => //.
   proc.
-  conseq (: _ ==> ={GAKEb_st.stop1}) _ (: _ ==> Counter.cis < q_is /\ Counter.cm1 < q_m1 /\ Counter.cm2 < q_m2) => //.
-  + call (A_res_bounded_qs (GAKEb_st(NTOR_S, NTOR_C, GAKEc.HROc.RO))).
+  conseq (: _ ==> ={UAKE_name_st.stop1}) _ (: _ ==> Counter.cis < q_is /\ Counter.cm1 < q_m1 /\ Counter.cm2 < q_m2) => //.
+  + call (A_res_bounded_qs (UAKE_name_st(NTOR_S, NTOR_C, UAKEc.HROc.RO))).
     by inline; auto.
   by sim. 
 fel
@@ -973,14 +968,14 @@ fel
   (Counter.cis + Counter.cm1 + Counter.cm2)
   (fun x => x%r / order%r)
   (q_m1 + q_m2 + q_is)
-  GAKEb_st.stop1
-  [ Counter(GAKEb_st(NTOR_S, NTOR_C, GAKEc.HROc.RO)).init_s : (arg \notin GAKEb_st.servers);
-    Counter(GAKEb_st(NTOR_S, NTOR_C, GAKEc.HROc.RO)).send_msg1 : ((arg.`2 \in GAKEb_st.servers) /\ ! get_sr_dh (oget GAKEb_st.servers.[arg.`2]) 
-                                /\ GAKEb_st.c_smap.[arg.`1] = None);
-    Counter(GAKEb_st(NTOR_S, NTOR_C, GAKEc.HROc.RO)).send_msg2 : (GAKEb_st.s_smap.[(arg.`1, arg.`2)] = None
-                                /\ exists v, obind get_skey GAKEb_st.servers.[arg.`1] = Some v)
+  UAKE_name_st.stop1
+  [ Counter(UAKE_name_st(NTOR_S, NTOR_C, UAKEc.HROc.RO)).init_s : (arg \notin UAKE_name_st.servers);
+    Counter(UAKE_name_st(NTOR_S, NTOR_C, UAKEc.HROc.RO)).send_msg1 : ((arg.`2 \in UAKE_name_st.servers) /\ ! get_sr_dh (oget UAKE_name_st.servers.[arg.`2]) 
+                                /\ UAKE_name_st.c_smap.[arg.`1] = None);
+    Counter(UAKE_name_st(NTOR_S, NTOR_C, UAKEc.HROc.RO)).send_msg2 : (UAKE_name_st.s_smap.[(arg.`1, arg.`2)] = None
+                                /\ exists v, obind get_skey UAKE_name_st.servers.[arg.`1] = Some v)
   ]
-  (card GAKEb_st.pk_set <= Counter.cis + Counter.cm1 + Counter.cm2 /\ 0 <= Counter.cis /\ 0 <= Counter.cm1 /\ 0 <= Counter.cm2)
+  (card UAKE_name_st.pk_set <= Counter.cis + Counter.cm1 + Counter.cm2 /\ 0 <= Counter.cis /\ 0 <= Counter.cm1 /\ 0 <= Counter.cm2)
 .
 + rewrite -mulr_suml StdBigop.Bigreal.sumidE.
   + smt(ge0_q_m1 ge0_q_m2 ge0_q_is).
@@ -992,11 +987,11 @@ fel
 + proc; inline.
   rcondt ^if; 1: auto => />.
   wp.
-  rnd (fun x => g ^ x \in GAKEb_st.pk_set).
+  rnd (fun x => g ^ x \in UAKE_name_st.pk_set).
   auto => />.
   move => &hr *.
-  apply (ler_trans (mu (dmap dt (fun x : ZModE.exp => g ^ x)) (mem GAKEb_st.pk_set{hr}))). 
-  + rewrite -(dmapE dt (fun x : ZModE.exp => g ^ x) (fun y => y \in GAKEb_st.pk_set{hr})).
+  apply (ler_trans (mu (dmap dt (fun x : ZModE.exp => g ^ x)) (mem UAKE_name_st.pk_set{hr}))). 
+  + rewrite -(dmapE dt (fun x : ZModE.exp => g ^ x) (fun y => y \in UAKE_name_st.pk_set{hr})).
     exact mu_le.
   rewrite (Mu_mem.mu_mem _ _ (1%r / order%r)).
   + move => x xin.
@@ -1022,11 +1017,11 @@ fel
   match None ^match; 1: auto => />.
   rcondt ^if; 1: auto => />.
   auto => />.
-  rnd (fun x => g ^ x \in GAKEb_st.pk_set).
+  rnd (fun x => g ^ x \in UAKE_name_st.pk_set).
   auto => />.
   move => &hr *.
-  apply (ler_trans (mu (dmap dt (fun x : ZModE.exp => g ^ x)) (mem GAKEb_st.pk_set{hr}))). 
-  + rewrite -(dmapE dt (fun x : ZModE.exp => g ^ x) (fun y => y \in GAKEb_st.pk_set{hr})).
+  apply (ler_trans (mu (dmap dt (fun x : ZModE.exp => g ^ x)) (mem UAKE_name_st.pk_set{hr}))). 
+  + rewrite -(dmapE dt (fun x : ZModE.exp => g ^ x) (fun y => y \in UAKE_name_st.pk_set{hr})).
     exact mu_le.
   rewrite (Mu_mem.mu_mem _ _ (1%r / order%r)).
   + move => x xin.
@@ -1064,12 +1059,12 @@ fel
   wp.
   swap ^r1<$ @ 1.
   wp.
-  rnd (fun x => g ^ x \in GAKEb_st.pk_set).
+  rnd (fun x => g ^ x \in UAKE_name_st.pk_set).
   auto => />.
   move => &hr 3? H *.
   split.
-  + apply (ler_trans (mu (dmap dt (fun x : ZModE.exp => g ^ x)) (mem GAKEb_st.pk_set{hr}))). 
-    + rewrite -(dmapE dt (fun x : ZModE.exp => g ^ x) (fun y => y \in GAKEb_st.pk_set{hr})).
+  + apply (ler_trans (mu (dmap dt (fun x : ZModE.exp => g ^ x)) (mem UAKE_name_st.pk_set{hr}))). 
+    + rewrite -(dmapE dt (fun x : ZModE.exp => g ^ x) (fun y => y \in UAKE_name_st.pk_set{hr})).
       exact mu_le.
     rewrite (Mu_mem.mu_mem _ _ (1%r / order%r)).
     + move => x xin.
@@ -1099,27 +1094,27 @@ fel
   by auto => /#. 
 qed.
 
-lemma bound_stop2 bit &m: Pr[GAKEc.E_GAKE_nodhs(GAKEb_st(NTOR_S, NTOR_C, GAKEc.HROc.RO), A_res).run(bit) @ &m : GAKEb_st.stop2] 
+lemma bound_stop2 bit &m: Pr[UAKEc.E_UAKE_RN(UAKE_name_st(NTOR_S, NTOR_C, UAKEc.HROc.RO), A_res).run(bit) @ &m : UAKE_name_st.stop2] 
   <= ((q_h + q_m1 + q_m2 + q_m3) * (q_h + q_m1 + q_m2 + q_m3 - 1))%r / (2 * order)%r.
 proof.
-have ->: Pr[E_GAKE_nodhs(GAKEb_st(NTOR_S, NTOR_C, GAKEc.HROc.RO), A_res).run(bit) @ &m : GAKEb_st.stop2]
-       = Pr[E_GAKE_nodhs(Counter(GAKEb_st(NTOR_S, NTOR_C, GAKEc.HROc.RO)), A_res).run(bit) @ &m : GAKEb_st.stop2].
+have ->: Pr[E_UAKE_RN(UAKE_name_st(NTOR_S, NTOR_C, UAKEc.HROc.RO), A_res).run(bit) @ &m : UAKE_name_st.stop2]
+       = Pr[E_UAKE_RN(Counter(UAKE_name_st(NTOR_S, NTOR_C, UAKEc.HROc.RO)), A_res).run(bit) @ &m : UAKE_name_st.stop2].
 + byequiv => //.
   proc.
-  call (: ={glob GAKEb_st, glob HROc.RO}); try (proc; inline; sim />).
+  call (: ={glob UAKE_name_st, glob HROc.RO}); try (proc; inline; sim />).
   + proc; inline. 
     by sp; if; auto.
   + by auto => />. 
   + by auto => />.
   + by auto => />.
   by inline; auto => />.
-have ->: Pr[E_GAKE_nodhs(Counter(GAKEb_st(NTOR_S, NTOR_C, GAKEc.HROc.RO)), A_res).run(bit) @ &m : GAKEb_st.stop2]
-       = Pr[E_GAKE_nodhs(Counter(GAKEb_st(NTOR_S, NTOR_C, GAKEc.HROc.RO)), A_res).run(bit) @ &m : GAKEb_st.stop2
+have ->: Pr[E_UAKE_RN(Counter(UAKE_name_st(NTOR_S, NTOR_C, UAKEc.HROc.RO)), A_res).run(bit) @ &m : UAKE_name_st.stop2]
+       = Pr[E_UAKE_RN(Counter(UAKE_name_st(NTOR_S, NTOR_C, UAKEc.HROc.RO)), A_res).run(bit) @ &m : UAKE_name_st.stop2
             /\ Counter.ch < q_h /\ Counter.cis < q_is /\ Counter.cm1 < q_m1 /\ Counter.cm2 < q_m2 /\ Counter.cm3 < q_m3].
 + byequiv => //.
   proc.
-  conseq (: _ ==> ={GAKEb_st.stop2}) _ (: _ ==> Counter.ch < q_h /\ Counter.cis < q_is /\ Counter.cm1 < q_m1 /\ Counter.cm2 < q_m2 /\ Counter.cm3 < q_m3) => //.
-  + call (A_res_bounded_qs (GAKEb_st(NTOR_S, NTOR_C, GAKEc.HROc.RO))).
+  conseq (: _ ==> ={UAKE_name_st.stop2}) _ (: _ ==> Counter.ch < q_h /\ Counter.cis < q_is /\ Counter.cm1 < q_m1 /\ Counter.cm2 < q_m2 /\ Counter.cm3 < q_m3) => //.
+  + call (A_res_bounded_qs (UAKE_name_st(NTOR_S, NTOR_C, UAKEc.HROc.RO))).
     by inline; auto.
   by sim. 
 fel
@@ -1127,16 +1122,16 @@ fel
   (Counter.ch + Counter.cm1 + Counter.cm2 + Counter.cm3)
   (fun x => x%r / order%r)
   (q_h + q_m1 + q_m2 + q_m3)
-  GAKEb_st.stop2
-  [ Counter(GAKEb_st(NTOR_S, NTOR_C, GAKEc.HROc.RO)).h : false;
-    Counter(GAKEb_st(NTOR_S, NTOR_C, GAKEc.HROc.RO)).init_s : false;
-    Counter(GAKEb_st(NTOR_S, NTOR_C, GAKEc.HROc.RO)).send_msg1 : ((arg.`2 \in GAKEb_st.servers) /\ ! get_sr_dh (oget GAKEb_st.servers.[arg.`2]) 
-                                /\ GAKEb_st.c_smap.[arg.`1] = None);
-    Counter(GAKEb_st(NTOR_S, NTOR_C, GAKEc.HROc.RO)).send_msg2 : (GAKEb_st.s_smap.[(arg.`1, arg.`2)] = None
-                                /\ exists v, obind get_skey GAKEb_st.servers.[arg.`1] = Some v);
-    Counter(GAKEb_st(NTOR_S, NTOR_C, GAKEc.HROc.RO)).send_msg3 : false
+  UAKE_name_st.stop2
+  [ Counter(UAKE_name_st(NTOR_S, NTOR_C, UAKEc.HROc.RO)).h : false;
+    Counter(UAKE_name_st(NTOR_S, NTOR_C, UAKEc.HROc.RO)).init_s : false;
+    Counter(UAKE_name_st(NTOR_S, NTOR_C, UAKEc.HROc.RO)).send_msg1 : ((arg.`2 \in UAKE_name_st.servers) /\ ! get_sr_dh (oget UAKE_name_st.servers.[arg.`2]) 
+                                /\ UAKE_name_st.c_smap.[arg.`1] = None);
+    Counter(UAKE_name_st(NTOR_S, NTOR_C, UAKEc.HROc.RO)).send_msg2 : (UAKE_name_st.s_smap.[(arg.`1, arg.`2)] = None
+                                /\ exists v, obind get_skey UAKE_name_st.servers.[arg.`1] = Some v);
+    Counter(UAKE_name_st(NTOR_S, NTOR_C, UAKEc.HROc.RO)).send_msg3 : false
   ]
-  (card GAKEb_st.x_set <= Counter.ch + Counter.cm2 /\ card GAKEb_st.y_set <= Counter.ch + Counter.cm3 /\ 0 <= Counter.ch /\ 0 <= Counter.cis /\ 0 <= Counter.cm1 /\ 0 <= Counter.cm2 /\ 0 <= Counter.cm3)
+  (card UAKE_name_st.x_set <= Counter.ch + Counter.cm2 /\ card UAKE_name_st.y_set <= Counter.ch + Counter.cm3 /\ 0 <= Counter.ch /\ 0 <= Counter.cis /\ 0 <= Counter.cm1 /\ 0 <= Counter.cm2 /\ 0 <= Counter.cm3)
 .
 + rewrite -mulr_suml StdBigop.Bigreal.sumidE.
   + smt(ge0_q_m1 ge0_q_m2 ge0_q_m3 ge0_q_h).
@@ -1173,11 +1168,11 @@ fel
   match None ^match; 1: auto => />.
   rcondt ^if; 1: auto => />.
   auto => />.
-  rnd (fun x => g ^ x \in GAKEb_st.x_set).
+  rnd (fun x => g ^ x \in UAKE_name_st.x_set).
   auto => />.
   move => &hr *.
-  apply (ler_trans (mu (dmap dt (fun x : ZModE.exp => g ^ x)) (mem GAKEb_st.x_set{hr}))). 
-  + rewrite -(dmapE dt (fun x : ZModE.exp => g ^ x) (fun y => y \in GAKEb_st.x_set{hr})).
+  apply (ler_trans (mu (dmap dt (fun x : ZModE.exp => g ^ x)) (mem UAKE_name_st.x_set{hr}))). 
+  + rewrite -(dmapE dt (fun x : ZModE.exp => g ^ x) (fun y => y \in UAKE_name_st.x_set{hr})).
     exact mu_le.
   rewrite (Mu_mem.mu_mem _ _ (1%r / order%r)).
   + move => x xin.
@@ -1215,12 +1210,12 @@ fel
   wp.
   swap ^r1<$ @ 1.
   wp. 
-  rnd (fun x => g ^ x \in GAKEb_st.y_set).
+  rnd (fun x => g ^ x \in UAKE_name_st.y_set).
   auto => />.
   move => &hr 4? H *.
   split.
-  + apply (ler_trans (mu (dmap dt (fun x : ZModE.exp => g ^ x)) (mem GAKEb_st.y_set{hr}))). 
-    + rewrite  (dmapE dt (fun x : ZModE.exp => g ^ x) (fun y => y \in GAKEb_st.y_set{hr})).
+  + apply (ler_trans (mu (dmap dt (fun x : ZModE.exp => g ^ x)) (mem UAKE_name_st.y_set{hr}))). 
+    + rewrite  (dmapE dt (fun x : ZModE.exp => g ^ x) (fun y => y \in UAKE_name_st.y_set{hr})).
       smt(in_fsetU1 mu_le).
     rewrite (Mu_mem.mu_mem _ _ (1%r / order%r)).
     + move => x xin.
@@ -1231,7 +1226,7 @@ fel
       rewrite duniform1E.
       rewrite DZmodP.Support.enumP /=.
       by rewrite undup_id 1:DZmodP.Support.enum_uniq -DZmodP.cardE.
-    have : (card GAKEb_st.y_set{hr})%r * (1%r / order%r) <= (Counter.ch{hr} + Counter.cm3{hr})%r / order%r.
+    have : (card UAKE_name_st.y_set{hr})%r * (1%r / order%r) <= (Counter.ch{hr} + Counter.cm3{hr})%r / order%r.
     + by move : H; clear; smt(gt0_order).
     smt(gt0_order).
   rewrite /get_as_Some //=.
@@ -1266,17 +1261,17 @@ qed.
 
 (* Unrestricted vs. restricted for the name-based model *)
 (* First restricted => unrestricted security *)
-lemma res_to_unres bit &m: Pr[GAKEc.E_GAKE_nodhs(GAKEc.GAKEb_nodhs(NTOR_S, NTOR_C, GAKEc.HROc.RO), A_res).run(bit) @ &m : res]
-  = Pr[GAKEc.E_GAKE(GAKEc.GAKEb(NTOR_S, NTOR_C, GAKEc.HROc.RO), Dh_Red(A_res)).run(bit) @ &m : res].
+lemma res_to_unres bit &m: Pr[UAKEc.E_UAKE_RN(UAKEc.O_RN(NTOR_S, NTOR_C, UAKEc.HROc.RO), A_res).run(bit) @ &m : res]
+  = Pr[UAKEc.E_UAKE_UN(UAKEc.O_UN(NTOR_S, NTOR_C, UAKEc.HROc.RO), Res_Red(A_res)).run(bit) @ &m : res].
 proof.
 byequiv => //.
 proc; inline.
-wp; call (: ={b0, servers, c_smap, s_smap, tested}(GAKEb_nodhs, GAKEc.GAKEb) /\ ={m}(GAKEc.HROc.RO, GAKEc.HROc.RO)
-              /\ (forall i s pt ir, i \in GAKEb.c_smap{2} => GAKEb.c_smap{2}.[i] = Some (Pending s pt ir)
-                   => pt.`1 \in GAKEb.servers{2})
-              /\ (forall i s t k ir, i \in GAKEb.c_smap{2} => GAKEb.c_smap{2}.[i] = Some (Accepted s t k ir) 
-                   => t.`1.`1 \in GAKEb.servers{2})
-              /\ (forall b, b \in GAKEb.servers{2} => ! get_sr_dh (oget GAKEb.servers{2}.[b]))); try sim />.
+wp; call (: ={b0, servers, c_smap, s_smap, tested}(O_RN, UAKEc.O_UN) /\ ={m}(UAKEc.HROc.RO, UAKEc.HROc.RO)
+              /\ (forall i s pt ir, i \in O_UN.c_smap{2} => O_UN.c_smap{2}.[i] = Some (Pending s pt ir)
+                   => pt.`1 \in O_UN.servers{2})
+              /\ (forall i s t k ir, i \in O_UN.c_smap{2} => O_UN.c_smap{2}.[i] = Some (Accepted s t k ir) 
+                   => t.`1.`1 \in O_UN.servers{2})
+              /\ (forall b, b \in O_UN.servers{2} => ! get_sr_dh (oget O_UN.servers{2}.[b]))); try sim />.
 
 + proc; inline.
   if => //.
@@ -1335,38 +1330,38 @@ smt(emptyE mem_empty).
 qed.
 
 (* Unrestricted => restricted security *)
-lemma gake_hon bit &m: Pr[GAKEc.E_GAKE(GAKEc.GAKEb(NTOR_S, NTOR_C, GAKEc.HROc.RO), A).run(bit) @ &m : res] 
-  = Pr[GAKEc.E_GAKE(GAKEc.GAKEb_hon(NTOR_S, NTOR_C, GAKEc.HROc.RO), Hon_Red(A)).run(bit) @ &m : res].
+lemma gake_hon bit &m: Pr[UAKEc.E_UAKE_UN(UAKEc.O_UN(NTOR_S, NTOR_C, UAKEc.HROc.RO), A).run(bit) @ &m : res] 
+  = Pr[UAKEc.E_UAKE_UN(UAKEc.O_HN(NTOR_S, NTOR_C, UAKEc.HROc.RO), Hon_Red(A)).run(bit) @ &m : res].
 proof.
 byequiv => //.
 proc; inline.
-wp; call (: ={b0, servers, s_smap, tested}(GAKEc.GAKEb, GAKEc.GAKEb_hon) /\ ={m}(GAKEc.HROc.RO, GAKEc.HROc.RO)
+wp; call (: ={b0, servers, s_smap, tested}(UAKEc.O_UN, UAKEc.O_HN) /\ ={m}(UAKEc.HROc.RO, UAKEc.HROc.RO)
   
-              /\ (GAKEc.GAKEb.c_smap{1} = (GAKEc.GAKEb_hon.c_smap{2} + Hon_Red.O_GAKE.dhc_smap{2}))
-              /\ (forall i, i \in Hon_Red.O_GAKE.dhc_smap{2} => i \notin GAKEc.GAKEb_hon.c_smap{2})
-              /\ (forall i, i \in GAKEc.GAKEb_hon.c_smap{2} => i \notin Hon_Red.O_GAKE.dhc_smap{2})
-              /\ (forall b, b \in Hon_Red.O_GAKE.servers{2} <=> b \in GAKEc.GAKEb_hon.servers{2})
-              /\ (forall b, b \in GAKEc.GAKEb_hon.servers{2} 
-                   => get_pkey (oget GAKEc.GAKEb_hon.servers{2}.[b]) = get_pkey_mod (oget Hon_Red.O_GAKE.servers{2}.[b])
-                                      /\ (get_sr_out (oget Hon_Red.O_GAKE.servers{2}.[b]) = get_sr_dh (oget GAKEc.GAKEb_hon.servers{2}.[b])))
-              /\ (forall i, i \in GAKEc.GAKEb.c_smap{1} <=> i \in Hon_Red.O_GAKE.c_inst{2})
-              /\ (forall i, i \in Hon_Red.O_GAKE.dhc_smap{2} => get_ir_test (oget Hon_Red.O_GAKE.dhc_smap{2}.[i]) = false
-                                       /\ get_name (oget Hon_Red.O_GAKE.dhc_smap{2}.[i]) \in GAKEb_hon.servers{2}
-                                       /\ get_sr_dh (oget GAKEb_hon.servers{2}.[get_name (oget Hon_Red.O_GAKE.dhc_smap{2}.[i])]))
-              /\ (forall b j , b \notin GAKEc.GAKEb_hon.servers{2} => (b, j) \notin GAKEc.GAKEb_hon.s_smap{2})
-              /\ (forall b j, (b, j) \in GAKEc.GAKEb_hon.s_smap{2} => get_name (oget GAKEc.GAKEb_hon.s_smap{2}.[(b, j)]) = b
-                                       /\ (exists pk m3, get_trace (oget GAKEc.GAKEb_hon.s_smap{2}.[(b, j)]) = Some ((b, pk), Some m3)))
-              /\ (forall b j, b \in GAKEc.GAKEb_hon.servers{2} => get_sr_dh (oget GAKEc.GAKEb_hon.servers{2}.[b])
-                   => (b, j) \notin GAKEc.GAKEb_hon.s_smap{2} /\ get_sr_ltk (oget GAKEc.GAKEb_hon.servers{2}.[b]))
-              /\ (forall i j, i \in Hon_Red.O_GAKE.dhc_smap{2}  
-                   => (get_name (oget Hon_Red.O_GAKE.dhc_smap{2}.[i]), j) \notin GAKEc.GAKEb_hon.s_smap{2})
-              /\ (forall i st pt ir m3, i \in Hon_Red.O_GAKE.dhc_smap{2} => Hon_Red.O_GAKE.dhc_smap{2}.[i] = Some (Pending st pt ir)
-                   => (1 <= card (get_partners_c (pt, Some m3) GAKEc.GAKEb_hon.s_smap{2})) = false)
-              /\ (forall i st pt ir, i \in Hon_Red.O_GAKE.dhc_smap{2} => Hon_Red.O_GAKE.dhc_smap{2}.[i] = Some (Pending st pt ir)
-                   => (1 <= card (get_origins_c (pt, None) GAKEc.GAKEb_hon.s_smap{2}) = false))
-              /\ (forall i st t k ir, i \in Hon_Red.O_GAKE.dhc_smap{2} => Hon_Red.O_GAKE.dhc_smap{2}.[i] = Some (Accepted st t k ir)
-                   => (1 <= card (get_origins_c t GAKEc.GAKEb_hon.s_smap{2}) = false)
-                          /\ (1 <= card (get_partners_c t GAKEc.GAKEb_hon.s_smap{2})) = false)).
+              /\ (UAKEc.O_UN.c_smap{1} = (UAKEc.O_HN.c_smap{2} + Hon_Red.O_UAKE_HN.dhc_smap{2}))
+              /\ (forall i, i \in Hon_Red.O_UAKE_HN.dhc_smap{2} => i \notin UAKEc.O_HN.c_smap{2})
+              /\ (forall i, i \in UAKEc.O_HN.c_smap{2} => i \notin Hon_Red.O_UAKE_HN.dhc_smap{2})
+              /\ (forall b, b \in Hon_Red.O_UAKE_HN.servers{2} <=> b \in UAKEc.O_HN.servers{2})
+              /\ (forall b, b \in UAKEc.O_HN.servers{2} 
+                   => get_pkey (oget UAKEc.O_HN.servers{2}.[b]) = get_pkey_mod (oget Hon_Red.O_UAKE_HN.servers{2}.[b])
+                                      /\ (get_sr_out (oget Hon_Red.O_UAKE_HN.servers{2}.[b]) = get_sr_dh (oget UAKEc.O_HN.servers{2}.[b])))
+              /\ (forall i, i \in UAKEc.O_UN.c_smap{1} <=> i \in Hon_Red.O_UAKE_HN.c_inst{2})
+              /\ (forall i, i \in Hon_Red.O_UAKE_HN.dhc_smap{2} => get_ir_test (oget Hon_Red.O_UAKE_HN.dhc_smap{2}.[i]) = false
+                                       /\ get_name (oget Hon_Red.O_UAKE_HN.dhc_smap{2}.[i]) \in O_HN.servers{2}
+                                       /\ get_sr_dh (oget O_HN.servers{2}.[get_name (oget Hon_Red.O_UAKE_HN.dhc_smap{2}.[i])]))
+              /\ (forall b j , b \notin UAKEc.O_HN.servers{2} => (b, j) \notin UAKEc.O_HN.s_smap{2})
+              /\ (forall b j, (b, j) \in UAKEc.O_HN.s_smap{2} => get_name (oget UAKEc.O_HN.s_smap{2}.[(b, j)]) = b
+                                       /\ (exists pk m3, get_trace (oget UAKEc.O_HN.s_smap{2}.[(b, j)]) = Some ((b, pk), Some m3)))
+              /\ (forall b j, b \in UAKEc.O_HN.servers{2} => get_sr_dh (oget UAKEc.O_HN.servers{2}.[b])
+                   => (b, j) \notin UAKEc.O_HN.s_smap{2} /\ get_sr_ltk (oget UAKEc.O_HN.servers{2}.[b]))
+              /\ (forall i j, i \in Hon_Red.O_UAKE_HN.dhc_smap{2}  
+                   => (get_name (oget Hon_Red.O_UAKE_HN.dhc_smap{2}.[i]), j) \notin UAKEc.O_HN.s_smap{2})
+              /\ (forall i st pt ir m3, i \in Hon_Red.O_UAKE_HN.dhc_smap{2} => Hon_Red.O_UAKE_HN.dhc_smap{2}.[i] = Some (Pending st pt ir)
+                   => (1 <= card (get_partners_c (pt, Some m3) UAKEc.O_HN.s_smap{2})) = false)
+              /\ (forall i st pt ir, i \in Hon_Red.O_UAKE_HN.dhc_smap{2} => Hon_Red.O_UAKE_HN.dhc_smap{2}.[i] = Some (Pending st pt ir)
+                   => (1 <= card (get_origins_c (pt, None) UAKEc.O_HN.s_smap{2}) = false))
+              /\ (forall i st t k ir, i \in Hon_Red.O_UAKE_HN.dhc_smap{2} => Hon_Red.O_UAKE_HN.dhc_smap{2}.[i] = Some (Accepted st t k ir)
+                   => (1 <= card (get_origins_c t UAKEc.O_HN.s_smap{2}) = false)
+                          /\ (1 <= card (get_partners_c t UAKEc.O_HN.s_smap{2})) = false)).
 
 + sim />.
 
@@ -1391,7 +1386,7 @@ wp; call (: ={b0, servers, s_smap, tested}(GAKEc.GAKEb, GAKEc.GAKEb_hon) /\ ={m}
     auto => />. 
   sp; match {1} => //.
   + rcondt {2} ^if. auto => /#.
-    auto => /> &2 ? ? ? ? ? ? ? ? inv ? ? ? ? ? ? ? sk *. do split; ~1,7,8: smt(get_setE mem_set in_fsetU1 joinE).
+    auto => /> &2 8? inv 7? sk *. do split; ~1,7,8: smt(get_setE mem_set in_fsetU1 joinE).
     + rewrite -fmap_eqP. smt(joinE get_setE).
     + move => i1 st0 pt ir0 m3.
       case (i1 = i{2}) => ieq; 2: smt(get_setE mem_set in_fsetU1).
@@ -1399,15 +1394,15 @@ wp; call (: ={b0, servers, s_smap, tested}(GAKEc.GAKEb, GAKEc.GAKEb_hon) /\ ={m}
       rewrite get_setE //=.
       move => [#] steq pteq ireq.
       rewrite /get_partners_c.
-      case ((i{2} \notin Hon_Red.O_GAKE.dhc_smap{2})) => indhc; 2: by smt(get_setE mem_set in_fsetU1 joinE).
-      have->: (fdom (filter (fun (_ : s_id * int) (val : GAKEc.pr_st_server GAKEc.instance_state) => get_trace val = Some (pt, Some m3)) GAKEb_hon.s_smap{2})) = fset0; 2: smt(fcards0).
+      case ((i{2} \notin Hon_Red.O_UAKE_HN.dhc_smap{2})) => indhc; 2: by smt(get_setE mem_set in_fsetU1 joinE).
+      have->: (fdom (filter (fun (_ : s_id * int) (val : UAKEc.s_state UAKEc.instance_state) => get_trace val = Some (pt, Some m3)) O_HN.s_smap{2})) = fset0; 2: smt(fcards0).
       rewrite fsetP.
       move => x.
       rewrite mem_fdom mem_filter.
-      have->: !(x \in GAKEb_hon.s_smap{2} /\ (fun (_ : s_id * int) (val : GAKEc.pr_st_server GAKEc.instance_state) =>
-              get_trace val = Some (pt, Some m3)) x (oget GAKEb_hon.s_smap{2}.[x])); 2: smt(get_setE in_fset0 joinE).
+      have->: !(x \in O_HN.s_smap{2} /\ (fun (_ : s_id * int) (val : UAKEc.s_state UAKEc.instance_state) =>
+              get_trace val = Some (pt, Some m3)) x (oget O_HN.s_smap{2}.[x])); 2: smt(get_setE in_fset0 joinE).
       rewrite negb_and.
-      case (x \in GAKEb_hon.s_smap{2}); 2: by smt().
+      case (x \in O_HN.s_smap{2}); 2: by smt().
       simplify.
       rewrite -pteq.
       move => xin.
@@ -1419,16 +1414,16 @@ wp; call (: ={b0, servers, s_smap, tested}(GAKEc.GAKEb, GAKEc.GAKEb_hon) /\ ={m}
     rewrite get_setE //=.
     move => [#] steq pteq ireq.
     rewrite /get_origins_c.
-    case ((i{2} \notin Hon_Red.O_GAKE.dhc_smap{2})) => indhc; 2: by smt(get_setE mem_set in_fsetU1 joinE).
-    have->: (fdom (filter (fun (_ : s_id * int) (val : GAKEc.pr_st_server GAKEc.instance_state) 
-          => exists (m2o : (pkey * tag) option), get_trace val = Some (pt, m2o)) GAKEb_hon.s_smap{2})) = fset0; 2: smt(fcards0).
+    case ((i{2} \notin Hon_Red.O_UAKE_HN.dhc_smap{2})) => indhc; 2: by smt(get_setE mem_set in_fsetU1 joinE).
+    have->: (fdom (filter (fun (_ : s_id * int) (val : UAKEc.s_state UAKEc.instance_state) 
+          => exists (m2o : (pkey * tag) option), get_trace val = Some (pt, m2o)) O_HN.s_smap{2})) = fset0; 2: smt(fcards0).
     rewrite fsetP.
     move => x.
     rewrite mem_fdom mem_filter. 
-    have->: !(x \in GAKEb_hon.s_smap{2} /\ (fun (_ : s_id * int) (val : GAKEc.pr_st_server GAKEc.instance_state) =>
-              exists (m2o : (pkey * tag) option), get_trace val = Some (pt, m2o)) x (oget GAKEb_hon.s_smap{2}.[x])); 2: smt(get_setE in_fset0 joinE).
+    have->: !(x \in O_HN.s_smap{2} /\ (fun (_ : s_id * int) (val : UAKEc.s_state UAKEc.instance_state) =>
+              exists (m2o : (pkey * tag) option), get_trace val = Some (pt, m2o)) x (oget O_HN.s_smap{2}.[x])); 2: smt(get_setE in_fset0 joinE).
     rewrite negb_and.
-    case (x \in GAKEb_hon.s_smap{2}); 2: by smt().
+    case (x \in O_HN.s_smap{2}); 2: by smt().
     simplify.
     rewrite -pteq.
     move => xin. 
@@ -1615,14 +1610,14 @@ wp; call (: ={b0, servers, s_smap, tested}(GAKEc.GAKEb, GAKEc.GAKEb_hon) /\ ={m}
         have := inv i{2} (b{2}, pk_b{2}, sk_ce{2}) pt ir iin stc.
         rewrite /get_origins_c //= => [#] H.
         split; 1: by rewrite H.
-        case (1 <= card (fdom (filter (fun (_ : s_id * int) (val : GAKEc.pr_st_server GAKEc.instance_state) =>
-               get_trace val = Some (pt, Some m3{2})) GAKEb_hon.s_smap{2}))) => p //=.
-        have : card (fdom (filter (fun (_ : s_id * int) (val : GAKEc.pr_st_server GAKEc.instance_state) =>
-                 get_trace val = Some (pt, Some m3{2})) GAKEb_hon.s_smap{2})) <> 0 by smt().
+        case (1 <= card (fdom (filter (fun (_ : s_id * int) (val : UAKEc.s_state UAKEc.instance_state) =>
+               get_trace val = Some (pt, Some m3{2})) O_HN.s_smap{2}))) => p //=.
+        have : card (fdom (filter (fun (_ : s_id * int) (val : UAKEc.s_state UAKEc.instance_state) =>
+                 get_trace val = Some (pt, Some m3{2})) O_HN.s_smap{2})) <> 0 by smt().
         rewrite fcard_eq0 => /mem_pick /mem_fdom.
         rewrite mem_filter.
-        have : card (fdom (filter (fun (_ : s_id * int) (val : GAKEc.pr_st_server GAKEc.instance_state) =>
-                 exists (m2o : (pkey * tag) option), get_trace val = Some (pt, m2o)) GAKEb_hon.s_smap{2})) = 0 by smt(fcard_ge0).
+        have : card (fdom (filter (fun (_ : s_id * int) (val : UAKEc.s_state UAKEc.instance_state) =>
+                 exists (m2o : (pkey * tag) option), get_trace val = Some (pt, m2o)) O_HN.s_smap{2})) = 0 by smt(fcard_ge0).
         rewrite fcard_eq0 => /fset0_nin.
         smt().
       auto => /> &1 &2 *. do split; ~1: smt(get_setE mem_set in_fsetU1).
@@ -1645,14 +1640,14 @@ wp; call (: ={b0, servers, s_smap, tested}(GAKEc.GAKEb, GAKEc.GAKEb_hon) /\ ={m}
       have := inv i{2} (b{2}, pk_b{2}, sk_ce{2}) pt ir iin stc.
       rewrite /get_origins_c //= => [#] H.
       split. by rewrite H.
-      case (1 <= card (fdom (filter (fun (_ : s_id * int) (val : GAKEc.pr_st_server GAKEc.instance_state) =>
-             get_trace val = Some (pt, Some m3{2})) GAKEb_hon.s_smap{2}))) => p //=. 
-      have : card (fdom (filter (fun (_ : s_id * int) (val : GAKEc.pr_st_server GAKEc.instance_state) =>
-               get_trace val = Some (pt, Some m3{2})) GAKEb_hon.s_smap{2})) <> 0 by smt().
+      case (1 <= card (fdom (filter (fun (_ : s_id * int) (val : UAKEc.s_state UAKEc.instance_state) =>
+             get_trace val = Some (pt, Some m3{2})) O_HN.s_smap{2}))) => p //=. 
+      have : card (fdom (filter (fun (_ : s_id * int) (val : UAKEc.s_state UAKEc.instance_state) =>
+               get_trace val = Some (pt, Some m3{2})) O_HN.s_smap{2})) <> 0 by smt().
       rewrite fcard_eq0 => /mem_pick /mem_fdom.
       rewrite mem_filter.
-      have : card (fdom (filter (fun (_ : s_id * int) (val : GAKEc.pr_st_server GAKEc.instance_state) =>
-               exists (m2o : (pkey * tag) option), get_trace val = Some (pt, m2o)) GAKEb_hon.s_smap{2})) = 0 by smt(fcard_ge0).
+      have : card (fdom (filter (fun (_ : s_id * int) (val : UAKEc.s_state UAKEc.instance_state) =>
+               exists (m2o : (pkey * tag) option), get_trace val = Some (pt, m2o)) O_HN.s_smap{2})) = 0 by smt(fcard_ge0).
       rewrite fcard_eq0 => /fset0_nin.
       smt().
     auto => /> &1 &2 *. do split; ~1: smt(get_setE mem_set in_fsetU1).  
@@ -1696,16 +1691,16 @@ wp; call (: ={b0, servers, s_smap, tested}(GAKEc.GAKEb, GAKEc.GAKEb_hon) /\ ={m}
   + auto => /> &1 &2 *. 
     rewrite /untested_partner_s.
     rewrite /get_partners_s /get_untested_partners_s.
-    have->: (fdom (filter (fun (_ : int) (val : GAKEc.pr_st_client GAKEc.instance_state) 
-             => get_trace val = Some t) (GAKEb_hon.c_smap{1} + Hon_Red.O_GAKE.dhc_smap{1}))) 
-        = (fdom (filter (fun (_ : int) (val : GAKEc.pr_st_client GAKEc.instance_state) => get_trace val = Some t) GAKEb_hon.c_smap{1})).
+    have->: (fdom (filter (fun (_ : int) (val : UAKEc.c_state UAKEc.instance_state) 
+             => get_trace val = Some t) (O_HN.c_smap{1} + Hon_Red.O_UAKE_HN.dhc_smap{1}))) 
+        = (fdom (filter (fun (_ : int) (val : UAKEc.c_state UAKEc.instance_state) => get_trace val = Some t) O_HN.c_smap{1})).
     + rewrite fsetP.
       move => x.
       do rewrite mem_fdom mem_filter.
       smt(joinE).
-    have->: (fdom (filter (fun (_ : int) (val : GAKEc.pr_st_client GAKEc.instance_state) => get_trace val = Some t /\ get_ir_test val = false)
-         (GAKEb_hon.c_smap{1} + Hon_Red.O_GAKE.dhc_smap{1}))) = (fdom (filter (fun (_ : int) (val : GAKEc.pr_st_client GAKEc.instance_state) =>
-            get_trace val = Some t /\ get_ir_test val = false) GAKEb_hon.c_smap{1})). 
+    have->: (fdom (filter (fun (_ : int) (val : UAKEc.c_state UAKEc.instance_state) => get_trace val = Some t /\ get_ir_test val = false)
+         (O_HN.c_smap{1} + Hon_Red.O_UAKE_HN.dhc_smap{1}))) = (fdom (filter (fun (_ : int) (val : UAKEc.c_state UAKEc.instance_state) =>
+            get_trace val = Some t /\ get_ir_test val = false) O_HN.c_smap{1})). 
     + rewrite fsetP.
       move => x.
       do rewrite mem_fdom mem_filter.
@@ -1746,20 +1741,20 @@ wp; call (: ={b0, servers, s_smap, tested}(GAKEc.GAKEb, GAKEc.GAKEb_hon) /\ ={m}
     move => kp. 
     if => //; 3: auto => />.
     + auto => /> &2 *.
-      have : (forall b j t, (b, j) \in GAKEc.GAKEb_hon.s_smap{2} /\ t = (oget (get_trace (oget GAKEc.GAKEb_hon.s_smap{2}.[b, j])))
-            => get_untested_partners_s t (GAKEb_hon.c_smap{2} + Hon_Red.O_GAKE.dhc_smap{2}) = get_untested_partners_s t GAKEc.GAKEb_hon.c_smap{2}
-            /\ get_partners_s t (GAKEb_hon.c_smap{2} + Hon_Red.O_GAKE.dhc_smap{2}) = get_partners_s t GAKEc.GAKEb_hon.c_smap{2}).
+      have : (forall b j t, (b, j) \in UAKEc.O_HN.s_smap{2} /\ t = (oget (get_trace (oget UAKEc.O_HN.s_smap{2}.[b, j])))
+            => get_untested_partners_s t (O_HN.c_smap{2} + Hon_Red.O_UAKE_HN.dhc_smap{2}) = get_untested_partners_s t UAKEc.O_HN.c_smap{2}
+            /\ get_partners_s t (O_HN.c_smap{2} + Hon_Red.O_UAKE_HN.dhc_smap{2}) = get_partners_s t UAKEc.O_HN.c_smap{2}).
       + rewrite /get_partners_s /get_untested_partners_s.
         move => b1 j t [] bjin teq.
-        have->: (fdom (filter (fun (_ : int) (val : GAKEc.pr_st_client GAKEc.instance_state) => get_trace val = Some t /\ get_ir_test val = false) (GAKEb_hon.c_smap{2} 
-              + Hon_Red.O_GAKE.dhc_smap{2}))) = (fdom (filter (fun (_ : int) (val : GAKEc.pr_st_client GAKEc.instance_state) 
-              => get_trace val = Some t /\ get_ir_test val = false) GAKEb_hon.c_smap{2})).
+        have->: (fdom (filter (fun (_ : int) (val : UAKEc.c_state UAKEc.instance_state) => get_trace val = Some t /\ get_ir_test val = false) (O_HN.c_smap{2} 
+              + Hon_Red.O_UAKE_HN.dhc_smap{2}))) = (fdom (filter (fun (_ : int) (val : UAKEc.c_state UAKEc.instance_state) 
+              => get_trace val = Some t /\ get_ir_test val = false) O_HN.c_smap{2})).
         + rewrite fsetP.
           move => x.
           do rewrite mem_fdom mem_filter.
           smt(joinE).
-        have->: (fdom (filter (fun (_ : int) (val : GAKEc.pr_st_client GAKEc.instance_state) => get_trace val = Some t) (GAKEb_hon.c_smap{2} + Hon_Red.O_GAKE.dhc_smap{2}))) = 
-              (fdom (filter (fun (_ : int) (val : GAKEc.pr_st_client GAKEc.instance_state) => get_trace val = Some t) GAKEb_hon.c_smap{2})). 
+        have->: (fdom (filter (fun (_ : int) (val : UAKEc.c_state UAKEc.instance_state) => get_trace val = Some t) (O_HN.c_smap{2} + Hon_Red.O_UAKE_HN.dhc_smap{2}))) = 
+              (fdom (filter (fun (_ : int) (val : UAKEc.c_state UAKEc.instance_state) => get_trace val = Some t) O_HN.c_smap{2})). 
         + rewrite fsetP.
           move => x.
           do rewrite mem_fdom mem_filter.
@@ -1796,7 +1791,7 @@ wp; call (: ={b0, servers, s_smap, tested}(GAKEc.GAKEb, GAKEc.GAKEb_hon) /\ ={m}
   if => //.
   + auto => /> &1 &2 *.
     split; 2: smt(joinE).
-    have->: tested_origins_c t GAKEb_hon.s_smap{1} = None.
+    have->: tested_origins_c t O_HN.s_smap{1} = None.
     + rewrite /tested_origins_c. smt(joinE).
     by smt().
   auto => /> &1 &2 *. do split; ~1: smt(get_setE mem_set in_fsetU1).  
@@ -1812,16 +1807,16 @@ wp; call (: ={b0, servers, s_smap, tested}(GAKEc.GAKEb, GAKEc.GAKEb_hon) /\ ={m}
   + auto => /> &1 &2 *. 
     rewrite /untested_partner_s.
     rewrite /get_partners_s /get_untested_partners_s.
-    have->: (fdom (filter (fun (_ : int) (val : GAKEc.pr_st_client GAKEc.instance_state) 
-               => get_trace val = Some t) (GAKEb_hon.c_smap{1} + Hon_Red.O_GAKE.dhc_smap{1}))) 
-      = (fdom (filter (fun (_ : int) (val : GAKEc.pr_st_client GAKEc.instance_state) => get_trace val = Some t) GAKEb_hon.c_smap{1})).
+    have->: (fdom (filter (fun (_ : int) (val : UAKEc.c_state UAKEc.instance_state) 
+               => get_trace val = Some t) (O_HN.c_smap{1} + Hon_Red.O_UAKE_HN.dhc_smap{1}))) 
+      = (fdom (filter (fun (_ : int) (val : UAKEc.c_state UAKEc.instance_state) => get_trace val = Some t) O_HN.c_smap{1})).
     + rewrite fsetP.
       move => x.
       do rewrite mem_fdom mem_filter.
       smt(joinE).
-    have->: (fdom (filter (fun (_ : int) (val : GAKEc.pr_st_client GAKEc.instance_state) => get_trace val = Some t /\ get_ir_test val = false)
-         (GAKEb_hon.c_smap{1} + Hon_Red.O_GAKE.dhc_smap{1}))) = (fdom (filter (fun (_ : int) (val : GAKEc.pr_st_client GAKEc.instance_state) =>
-            get_trace val = Some t /\ get_ir_test val = false) GAKEb_hon.c_smap{1})). 
+    have->: (fdom (filter (fun (_ : int) (val : UAKEc.c_state UAKEc.instance_state) => get_trace val = Some t /\ get_ir_test val = false)
+         (O_HN.c_smap{1} + Hon_Red.O_UAKE_HN.dhc_smap{1}))) = (fdom (filter (fun (_ : int) (val : UAKEc.c_state UAKEc.instance_state) =>
+            get_trace val = Some t /\ get_ir_test val = false) O_HN.c_smap{1})). 
     + rewrite fsetP.
       move => x.
       do rewrite mem_fdom mem_filter.
@@ -1886,20 +1881,20 @@ wp; call (: ={b0, servers, s_smap, tested}(GAKEc.GAKEb, GAKEc.GAKEb_hon) /\ ={m}
     + auto => /> &1 &2 *.
       rewrite /fresh_partner_s.
       rewrite /get_origins_s /get_fresh_partners_s.
-      have->: (fdom (filter (fun (_ : int) (val : GAKEc.pr_st_client GAKEc.instance_state) =>
-             exists (m2o : (pkey * tag) option), get_trace val = Some (t.`1, m2o)) (GAKEb_hon.c_smap{1} + Hon_Red.O_GAKE.dhc_smap{1}))) = (fdom
-             (filter (fun (_ : int) (val : GAKEc.pr_st_client GAKEc.instance_state) => exists (m2o : (pkey * tag) option), get_trace val 
-             = Some (t.`1, m2o)) GAKEb_hon.c_smap{1})).
+      have->: (fdom (filter (fun (_ : int) (val : UAKEc.c_state UAKEc.instance_state) =>
+             exists (m2o : (pkey * tag) option), get_trace val = Some (t.`1, m2o)) (O_HN.c_smap{1} + Hon_Red.O_UAKE_HN.dhc_smap{1}))) = (fdom
+             (filter (fun (_ : int) (val : UAKEc.c_state UAKEc.instance_state) => exists (m2o : (pkey * tag) option), get_trace val 
+             = Some (t.`1, m2o)) O_HN.c_smap{1})).
       + rewrite fsetP.
         move => x.
         do rewrite mem_fdom mem_filter.
         smt(joinE).
-      have->: (fdom (filter (fun (_ : int) (val : GAKEc.pr_st_client GAKEc.instance_state) =>
+      have->: (fdom (filter (fun (_ : int) (val : UAKEc.c_state UAKEc.instance_state) =>
                 (exists (m2o : (pkey * tag) option), get_trace val = Some (t.`1, m2o)) /\ get_ir_test val = false /\ get_ir_sess val 
                   = false /\ get_ir_eph val = false)
-             (GAKEb_hon.c_smap{1} + Hon_Red.O_GAKE.dhc_smap{1}))) = (fdom (filter (fun (_ : int) (val : GAKEc.pr_st_client GAKEc.instance_state) =>
+             (O_HN.c_smap{1} + Hon_Red.O_UAKE_HN.dhc_smap{1}))) = (fdom (filter (fun (_ : int) (val : UAKEc.c_state UAKEc.instance_state) =>
                 (exists (m2o : (pkey * tag) option), get_trace val = Some (t.`1, m2o)) /\ get_ir_test val = false 
-                    /\ get_ir_sess val = false /\ get_ir_eph val = false) GAKEb_hon.c_smap{1})). 
+                    /\ get_ir_sess val = false /\ get_ir_eph val = false) O_HN.c_smap{1})). 
       + rewrite fsetP.
         move => x.
         do rewrite mem_fdom mem_filter.
@@ -1975,28 +1970,28 @@ wp; call (: ={b0, servers, s_smap, tested}(GAKEc.GAKEb, GAKEc.GAKEb_hon) /\ ={m}
 auto => />; smt(fmap_eqP joinE mem_empty emptyE).
 qed.
 
-lemma gake_rem_dhs bit &m: Pr[GAKEc.E_GAKE(GAKEc.GAKEb_hon(NTOR_S, NTOR_C, GAKEc.HROc.RO), Hon_Red(A)).run(bit) @ &m : res] 
- = Pr[GAKEc.E_GAKE_nodhs(GAKEc.GAKEb_nodhs(NTOR_S, NTOR_C, GAKEc.HROc.RO), Hon_s_Red(Hon_Red(A))).run(bit) @ &m : res].
+lemma gake_rem_dhs bit &m: Pr[UAKEc.E_UAKE_UN(UAKEc.O_HN(NTOR_S, NTOR_C, UAKEc.HROc.RO), Hon_Red(A)).run(bit) @ &m : res] 
+ = Pr[UAKEc.E_UAKE_RN(UAKEc.O_RN(NTOR_S, NTOR_C, UAKEc.HROc.RO), Hon_s_Red(Hon_Red(A))).run(bit) @ &m : res].
 proof. 
 byequiv => //.
 proc; inline.
-wp; call (: ={b0, c_smap, s_smap, tested}(GAKEb_hon, GAKEc.GAKEb_nodhs) /\ ={m}(GAKEc.HROc.RO, GAKEc.HROc.RO) /\ ={glob Hon_Red}
-               /\ (forall b, b \in GAKEb_hon.servers{1} <=> b \in Hon_s_Red.O_GAKE.servers{2})
-               /\ (forall b, b \in GAKEb_hon.servers{1} <=> b \in Hon_Red.O_GAKE.servers{1})
-               /\ (forall b, b \notin Hon_s_Red.O_GAKE.servers{2} => b \notin GAKEc.GAKEb_nodhs.servers{2})
-               /\ (forall b, b \in Hon_Red.O_GAKE.servers{1} => ! get_sr_out (oget Hon_Red.O_GAKE.servers{1}.[b])
-                    => b \in GAKEb_nodhs.servers{2})
-               /\ (forall b, b \in GAKEb_nodhs.servers{2} => !get_sr_dh (oget GAKEb_nodhs.servers{2}.[b]))
-               /\ (forall b, b \in GAKEb_hon.servers{1} => ! get_sr_dh (oget GAKEb_hon.servers{1}.[b])
-                    => GAKEb_hon.servers{1}.[b] = GAKEc.GAKEb_nodhs.servers{2}.[b])
-               /\ (forall b, b \in GAKEc.GAKEb_nodhs.servers{2} => ! get_sr_dh (oget GAKEc.GAKEb_nodhs.servers{2}.[b])
-                    /\ ! get_sr_dh (oget GAKEb_hon.servers{1}.[b])
-                    /\ (! get_sr_ltk (oget GAKEc.GAKEb_nodhs.servers{2}.[b]) <=> ! get_sr_ltk (oget GAKEb_hon.servers{1}.[b])))
-               /\ (forall b, get_sr_dh (oget GAKEb_hon.servers{1}.[b]) => get_sr_ltk (oget GAKEb_hon.servers{1}.[b]))
-               /\ (forall b, get_sr_dh (oget GAKEc.GAKEb_nodhs.servers{2}.[b]) => get_sr_ltk (oget GAKEc.GAKEb_nodhs.servers{2}.[b]))
-               /\ (forall b, b \in Hon_s_Red.O_GAKE.servers{2} => omap get_pkey GAKEb_hon.servers{1}.[b] = (oget Hon_s_Red.O_GAKE.servers{2}.[b]).`2)
-               /\ (forall i, i \in GAKEc.GAKEb_nodhs.c_smap{2} => get_name (oget GAKEc.GAKEb_nodhs.c_smap{2}.[i]) \in GAKEc.GAKEb_nodhs.servers{2})
-               /\ (forall b j, (b, j) \in GAKEc.GAKEb_nodhs.s_smap{2} => b \in GAKEc.GAKEb_nodhs.servers{2})
+wp; call (: ={b0, c_smap, s_smap, tested}(O_HN, UAKEc.O_RN) /\ ={m}(UAKEc.HROc.RO, UAKEc.HROc.RO) /\ ={glob Hon_Red}
+               /\ (forall b, b \in O_HN.servers{1} <=> b \in Hon_s_Red.O_UAKE.servers{2})
+               /\ (forall b, b \in O_HN.servers{1} <=> b \in Hon_Red.O_UAKE_HN.servers{1})
+               /\ (forall b, b \notin Hon_s_Red.O_UAKE.servers{2} => b \notin UAKEc.O_RN.servers{2})
+               /\ (forall b, b \in Hon_Red.O_UAKE_HN.servers{1} => ! get_sr_out (oget Hon_Red.O_UAKE_HN.servers{1}.[b])
+                    => b \in O_RN.servers{2})
+               /\ (forall b, b \in O_RN.servers{2} => !get_sr_dh (oget O_RN.servers{2}.[b]))
+               /\ (forall b, b \in O_HN.servers{1} => ! get_sr_dh (oget O_HN.servers{1}.[b])
+                    => O_HN.servers{1}.[b] = UAKEc.O_RN.servers{2}.[b])
+               /\ (forall b, b \in UAKEc.O_RN.servers{2} => ! get_sr_dh (oget UAKEc.O_RN.servers{2}.[b])
+                    /\ ! get_sr_dh (oget O_HN.servers{1}.[b])
+                    /\ (! get_sr_ltk (oget UAKEc.O_RN.servers{2}.[b]) <=> ! get_sr_ltk (oget O_HN.servers{1}.[b])))
+               /\ (forall b, get_sr_dh (oget O_HN.servers{1}.[b]) => get_sr_ltk (oget O_HN.servers{1}.[b]))
+               /\ (forall b, get_sr_dh (oget UAKEc.O_RN.servers{2}.[b]) => get_sr_ltk (oget UAKEc.O_RN.servers{2}.[b]))
+               /\ (forall b, b \in Hon_s_Red.O_UAKE.servers{2} => omap get_pkey O_HN.servers{1}.[b] = (oget Hon_s_Red.O_UAKE.servers{2}.[b]).`2)
+               /\ (forall i, i \in UAKEc.O_RN.c_smap{2} => get_name (oget UAKEc.O_RN.c_smap{2}.[i]) \in UAKEc.O_RN.servers{2})
+               /\ (forall b j, (b, j) \in UAKEc.O_RN.s_smap{2} => b \in UAKEc.O_RN.servers{2})
       ); 1: sim />.
 
 + proc; inline.
@@ -2111,10 +2106,10 @@ wp; call (: ={b0, c_smap, s_smap, tested}(GAKEb_hon, GAKEc.GAKEb_nodhs) /\ ={m}(
     do rewrite negb_or.
     rewrite /fresh_partner_c.
     rewrite /get_fresh_partners_c.
-    have->: (fdom (filter (fun (_ : s_id * int) (val : GAKEc.pr_st_server GAKEc.instance_state) => get_trace val = Some t /\ get_ir_test val = false 
-              /\ get_ir_sess val = false /\ (get_ir_eph val = false \/ get_sr_ltk (oget GAKEb_hon.servers{1}.[t.`1.`1]) = false)) GAKEb_hon.s_smap{1})) 
-          = (fdom (filter (fun (_ : s_id * int) (val : GAKEc.pr_st_server GAKEc.instance_state) => get_trace val = Some t /\ get_ir_test val = false 
-              /\ get_ir_sess val = false /\ (get_ir_eph val = false \/ get_sr_ltk (oget GAKEb_nodhs.servers{2}.[t.`1.`1]) = false)) GAKEb_nodhs.s_smap{2})).
+    have->: (fdom (filter (fun (_ : s_id * int) (val : UAKEc.s_state UAKEc.instance_state) => get_trace val = Some t /\ get_ir_test val = false 
+              /\ get_ir_sess val = false /\ (get_ir_eph val = false \/ get_sr_ltk (oget O_HN.servers{1}.[t.`1.`1]) = false)) O_HN.s_smap{1})) 
+          = (fdom (filter (fun (_ : s_id * int) (val : UAKEc.s_state UAKEc.instance_state) => get_trace val = Some t /\ get_ir_test val = false 
+              /\ get_ir_sess val = false /\ (get_ir_eph val = false \/ get_sr_ltk (oget O_RN.servers{2}.[t.`1.`1]) = false)) O_RN.s_smap{2})).
     + rewrite fsetP. 
       move => x.
       do rewrite mem_fdom mem_filter. smt(get_setE mem_set).
@@ -2133,20 +2128,20 @@ wp; call (: ={b0, c_smap, s_smap, tested}(GAKEb_hon, GAKEc.GAKEb_nodhs) /\ ={m}(
     do rewrite negb_or.
     rewrite /fresh_partner_s.
     rewrite /get_origins_s /get_fresh_partners_s.
-    have->: (fdom (filter (fun (_ : int) (val : GAKEc.pr_st_client GAKEc.instance_state) =>  exists (m2o : (pkey * tag) option), get_trace val 
-              = Some (t.`1, m2o)) GAKEb_hon.c_smap{1})) = (fdom (filter (fun (_ : int) (val : GAKEc.pr_st_client GAKEc.instance_state) =>
-                 exists (m2o : (pkey * tag) option), get_trace val = Some (t.`1, m2o)) GAKEb_nodhs.c_smap{2})).
+    have->: (fdom (filter (fun (_ : int) (val : UAKEc.c_state UAKEc.instance_state) =>  exists (m2o : (pkey * tag) option), get_trace val 
+              = Some (t.`1, m2o)) O_HN.c_smap{1})) = (fdom (filter (fun (_ : int) (val : UAKEc.c_state UAKEc.instance_state) =>
+                 exists (m2o : (pkey * tag) option), get_trace val = Some (t.`1, m2o)) O_RN.c_smap{2})).
     + rewrite fsetP. 
       move => x.
       do rewrite mem_fdom mem_filter. smt(get_setE mem_set).
-    have->: (fdom (filter (fun (_ : int) (val : GAKEc.pr_st_client GAKEc.instance_state) => (exists (m2o : (pkey * tag) option), get_trace val 
-              = Some (t.`1, m2o)) /\ get_ir_test val = false /\  get_ir_sess val = false /\ get_ir_eph val = false) GAKEb_hon.c_smap{1}))
-            = (fdom (filter (fun (_ : int) (val : GAKEc.pr_st_client GAKEc.instance_state) => (exists (m2o : (pkey * tag) option), get_trace val 
-              = Some (t.`1, m2o)) /\ get_ir_test val = false /\ get_ir_sess val = false /\ get_ir_eph val = false) GAKEb_nodhs.c_smap{2})).
+    have->: (fdom (filter (fun (_ : int) (val : UAKEc.c_state UAKEc.instance_state) => (exists (m2o : (pkey * tag) option), get_trace val 
+              = Some (t.`1, m2o)) /\ get_ir_test val = false /\  get_ir_sess val = false /\ get_ir_eph val = false) O_HN.c_smap{1}))
+            = (fdom (filter (fun (_ : int) (val : UAKEc.c_state UAKEc.instance_state) => (exists (m2o : (pkey * tag) option), get_trace val 
+              = Some (t.`1, m2o)) /\ get_ir_test val = false /\ get_ir_sess val = false /\ get_ir_eph val = false) O_RN.c_smap{2})).
     + rewrite fsetP. 
       move => x.
       do rewrite mem_fdom mem_filter. smt(get_setE mem_set).
-    have->: get_sr_ltk (oget GAKEb_hon.servers{1}.[b0{1}]) = get_sr_ltk (oget GAKEb_nodhs.servers{2}.[b0{2}]) by smt().
+    have->: get_sr_ltk (oget O_HN.servers{1}.[b0{1}]) = get_sr_ltk (oget O_RN.servers{2}.[b0{2}]) by smt().
     smt(get_setE mem_set).
   + if => //; auto => />; smt(get_setE mem_set).
   auto => />.
@@ -2155,8 +2150,8 @@ auto => />. smt(mem_empty emptyE).
 qed.
 
 
-lemma unres_to_res bit &m: Pr[GAKEc.E_GAKE(GAKEc.GAKEb(NTOR_S, NTOR_C, GAKEc.HROc.RO), A).run(bit) @ &m : res] 
-  = Pr[GAKEc.E_GAKE_nodhs(GAKEc.GAKEb_nodhs(NTOR_S, NTOR_C, GAKEc.HROc.RO), Hon_s_Red(Hon_Red(A))).run(bit) @ &m : res].
+lemma unres_to_res bit &m: Pr[UAKEc.E_UAKE_UN(UAKEc.O_UN(NTOR_S, NTOR_C, UAKEc.HROc.RO), A).run(bit) @ &m : res] 
+  = Pr[UAKEc.E_UAKE_RN(UAKEc.O_RN(NTOR_S, NTOR_C, UAKEc.HROc.RO), Hon_s_Red(Hon_Red(A))).run(bit) @ &m : res].
 proof.
 by rewrite gake_hon -gake_rem_dhs. 
 qed.
@@ -2164,12 +2159,12 @@ qed.
 
 (* Names vs. Public keys in the restricted model *)
 (* We only do reduction from restricted name-based model to restricted public-key-only model *)
-local lemma gake_st bit &m: Pr[GAKEc.E_GAKE_nodhs(GAKEc.GAKEb_nodhs(NTOR_S, NTOR_C, GAKEc.HROc.RO), A_res).run(bit) @ &m : res] 
-                = Pr[GAKEc.E_GAKE_nodhs(GAKEb_st(NTOR_S, NTOR_C, GAKEc.HROc.RO), A_res).run(bit) @ &m : res].
+local lemma gake_st bit &m: Pr[UAKEc.E_UAKE_RN(UAKEc.O_RN(NTOR_S, NTOR_C, UAKEc.HROc.RO), A_res).run(bit) @ &m : res] 
+                = Pr[UAKEc.E_UAKE_RN(UAKE_name_st(NTOR_S, NTOR_C, UAKEc.HROc.RO), A_res).run(bit) @ &m : res].
 proof.
 byequiv => //.
 proc; inline.
-wp; call (: ={b0, servers, c_smap, s_smap, tested}(GAKEc.GAKEb_nodhs, GAKEb_st) /\ ={m}(GAKEc.HROc.RO, GAKEc.HROc.RO)); try sim />.
+wp; call (: ={b0, servers, c_smap, s_smap, tested}(UAKEc.O_RN, UAKE_name_st) /\ ={m}(UAKEc.HROc.RO, UAKEc.HROc.RO)); try sim />.
 
 proc; inline.
 auto => />.
@@ -2186,14 +2181,14 @@ by rewrite /image /card -(perm_eq_size _ _ uniq_f) size_map.
 qed.
 
 
-op rem_sid_c (s : GAKEc.pr_st_client GAKEc.instance_state) : GAKE_mod.pr_st_client GAKE_mod.instance_state =
+op rem_sid_c (s : UAKEc.c_state UAKEc.instance_state) : UAKE_mod.c_state UAKE_mod.instance_state =
 match s with 
 | Pending st pt ir => Pending_mod (st.`2, st.`3) (st.`2, pt.`2) ir
 | Accepted st t k ir => Accepted_mod (st.`2, st.`3) ((st.`2, (t.`1).`2), t.`2) k ir
 | Aborted st t ir => Aborted_mod (Some ((oget st).`2, (oget st).`3)) (Some (((oget st).`2, ((oget t).`1).`2), (oget t).`2)) ir
 end.
 
-op rem_sid_s (s : GAKEc.pr_st_server GAKEc.instance_state) : GAKE_mod.pr_st_server GAKE_mod.instance_state =
+op rem_sid_s (s : UAKEc.s_state UAKEc.instance_state) : UAKE_mod.s_state UAKE_mod.instance_state =
 match s with 
 | Pending st pt ir => Pending_mod (st.`2, st.`3) (g ^ st.`2, pt.`2) ir
 | Accepted st t k ir => Accepted_mod (st.`2, st.`3) ((g ^ st.`2, (t.`1).`2), t.`2) k ir
@@ -2201,94 +2196,94 @@ match s with
 end.
 
 
-local lemma gake_no_name bit &m: `| Pr[GAKEc.E_GAKE_nodhs(GAKEb_st(NTOR_S, NTOR_C, GAKEc.HROc.RO), A_res).run(bit) @ &m : res]
-     - Pr[GAKE_mod.E_GAKE_nodhs(GAKE_mod.GAKEb_nodhs(NTOR_S_mod, NTOR_C_mod, GAKE_mod.HROc.RO), Name_Red(A_res)).run(bit) @ &m : res] | 
-                 <= Pr[GAKEc.E_GAKE_nodhs(GAKEb_st(NTOR_S, NTOR_C, GAKEc.HROc.RO), A_res).run(bit) @ &m : (GAKEb_st.stop1 \/ GAKEb_st.stop2)].
+local lemma gake_no_name bit &m: `| Pr[UAKEc.E_UAKE_RN(UAKE_name_st(NTOR_S, NTOR_C, UAKEc.HROc.RO), A_res).run(bit) @ &m : res]
+     - Pr[UAKE_mod.E_UAKE(UAKE_mod.O_RPK(S, C, UAKE_mod.HROc.RO), Name_Red(A_res)).run(bit) @ &m : res] | 
+                 <= Pr[UAKEc.E_UAKE_RN(UAKE_name_st(NTOR_S, NTOR_C, UAKEc.HROc.RO), A_res).run(bit) @ &m : (UAKE_name_st.stop1 \/ UAKE_name_st.stop2)].
 proof. 
 rewrite StdOrder.RealOrder.distrC.
-byequiv (: _ ==> _) : (Name_Red.O_GAKE.stop1 \/  Name_Red.O_GAKE.stop2) => //; first last.
+byequiv (: _ ==> _) : (Name_Red.O_UAKE_RN.stop1 \/  Name_Red.O_UAKE_RN.stop2) => //; first last.
 + smt().
 symmetry; proc; inline.
-wp; call (: (Name_Red.O_GAKE.stop1 \/  Name_Red.O_GAKE.stop2)
-          , ={b0, tested}(GAKEb_st, GAKE_mod.GAKEb_nodhs) /\ ={pk_set, x_set, y_set, stop1, stop2}(GAKEb_st, Name_Red.O_GAKE)
+wp; call (: (Name_Red.O_UAKE_RN.stop1 \/  Name_Red.O_UAKE_RN.stop2)
+          , ={b0, tested}(UAKE_name_st, UAKE_mod.O_RPK) /\ ={pk_set, x_set, y_set, stop1, stop2}(UAKE_name_st, Name_Red.O_UAKE_RN)
 
-               /\ (forall x, x \in GAKEc.HROc.RO.m{1} => x.`3 \in Name_Red.O_GAKE.sid_pk{2} => x \notin Name_Red.O_GAKE.unreg_ro{2}
-                    => GAKEc.HROc.RO.m{1}.[x] = GAKE_mod.HROc.RO.m{2}.[(x.`1, x.`2, (oget Name_Red.O_GAKE.sid_pk{2}.[x.`3]), x.`4, x.`5)])
-               /\ (forall x, x \in GAKEc.HROc.RO.m{1} => x.`3 \notin Name_Red.O_GAKE.sid_pk{2} => x \in Name_Red.O_GAKE.unreg_ro{2})
-               /\ (forall x, x \notin GAKEc.HROc.RO.m{1} => x.`3 \in Name_Red.O_GAKE.sid_pk{2}
-                    => (x.`1, x.`2, (oget Name_Red.O_GAKE.sid_pk{2}.[x.`3]), x.`4, x.`5) \notin GAKE_mod.HROc.RO.m{2})
-               /\ (forall x, x \in Name_Red.O_GAKE.unreg_ro{2} => x \in GAKEc.HROc.RO.m{1} /\ Name_Red.O_GAKE.unreg_ro{2}.[x] = GAKEc.HROc.RO.m{1}.[x])
-               /\ (forall x, x \in GAKEb_st.unreg_ro{1} <=> x \in Name_Red.O_GAKE.unreg_ro{2})
-               /\ (forall x, x \in GAKEc.HROc.RO.m{1} => x \in Name_Red.O_GAKE.unreg_ro{2} 
-                         \/ (x.`3 \in Name_Red.O_GAKE.sid_pk{2} /\ (x.`1, x.`2, (oget Name_Red.O_GAKE.sid_pk{2}.[x.`3]), x.`4, x.`5) \in GAKE_mod.HROc.RO.m{2}))
-               /\ (forall x, x \in Name_Red.O_GAKE.unreg_ro{2} => x.`3 \in Name_Red.O_GAKE.sid_pk{2} 
-                    => (x.`1, x.`2, (oget Name_Red.O_GAKE.sid_pk{2}.[x.`3]), x.`4, x.`5) \notin GAKE_mod.HROc.RO.m{2})
-               /\ (forall x, x \in GAKE_mod.HROc.RO.m{2} => (exists b, b \in Name_Red.O_GAKE.sid_pk{2} /\ Name_Red.O_GAKE.sid_pk{2}.[b] = Some x.`3 
-                                     /\ (x.`1, x.`2, b, x.`4, x.`5) \notin Name_Red.O_GAKE.unreg_ro{2}))
-               /\ (forall x, x \in GAKEc.HROc.RO.m{1} => (x.`4 \in Name_Red.O_GAKE.x_set{2} \/ x.`4 \in Name_Red.O_GAKE.pk_set{2}) 
-                                     /\ (x.`5 \in Name_Red.O_GAKE.y_set{2} \/ x.`5 \in Name_Red.O_GAKE.pk_set{2}))
-               /\ (forall x, x \in GAKE_mod.HROc.RO.m{2} => (x.`4 \in Name_Red.O_GAKE.x_set{2} \/ x.`4 \in Name_Red.O_GAKE.pk_set{2}) 
-                                     /\ (x.`5 \in Name_Red.O_GAKE.y_set{2} \/ x.`5 \in Name_Red.O_GAKE.pk_set{2}))
-               /\ (forall x, x \in Name_Red.O_GAKE.unreg_ro{2} => x.`4 \in Name_Red.O_GAKE.x_set{2} /\ x.`5 \in Name_Red.O_GAKE.y_set{2})
+               /\ (forall x, x \in UAKEc.HROc.RO.m{1} => x.`3 \in Name_Red.O_UAKE_RN.sid_pk{2} => x \notin Name_Red.O_UAKE_RN.unreg_ro{2}
+                    => UAKEc.HROc.RO.m{1}.[x] = UAKE_mod.HROc.RO.m{2}.[(x.`1, x.`2, (oget Name_Red.O_UAKE_RN.sid_pk{2}.[x.`3]), x.`4, x.`5)])
+               /\ (forall x, x \in UAKEc.HROc.RO.m{1} => x.`3 \notin Name_Red.O_UAKE_RN.sid_pk{2} => x \in Name_Red.O_UAKE_RN.unreg_ro{2})
+               /\ (forall x, x \notin UAKEc.HROc.RO.m{1} => x.`3 \in Name_Red.O_UAKE_RN.sid_pk{2}
+                    => (x.`1, x.`2, (oget Name_Red.O_UAKE_RN.sid_pk{2}.[x.`3]), x.`4, x.`5) \notin UAKE_mod.HROc.RO.m{2})
+               /\ (forall x, x \in Name_Red.O_UAKE_RN.unreg_ro{2} => x \in UAKEc.HROc.RO.m{1} /\ Name_Red.O_UAKE_RN.unreg_ro{2}.[x] = UAKEc.HROc.RO.m{1}.[x])
+               /\ (forall x, x \in UAKE_name_st.unreg_ro{1} <=> x \in Name_Red.O_UAKE_RN.unreg_ro{2})
+               /\ (forall x, x \in UAKEc.HROc.RO.m{1} => x \in Name_Red.O_UAKE_RN.unreg_ro{2} 
+                         \/ (x.`3 \in Name_Red.O_UAKE_RN.sid_pk{2} /\ (x.`1, x.`2, (oget Name_Red.O_UAKE_RN.sid_pk{2}.[x.`3]), x.`4, x.`5) \in UAKE_mod.HROc.RO.m{2}))
+               /\ (forall x, x \in Name_Red.O_UAKE_RN.unreg_ro{2} => x.`3 \in Name_Red.O_UAKE_RN.sid_pk{2} 
+                    => (x.`1, x.`2, (oget Name_Red.O_UAKE_RN.sid_pk{2}.[x.`3]), x.`4, x.`5) \notin UAKE_mod.HROc.RO.m{2})
+               /\ (forall x, x \in UAKE_mod.HROc.RO.m{2} => (exists b, b \in Name_Red.O_UAKE_RN.sid_pk{2} /\ Name_Red.O_UAKE_RN.sid_pk{2}.[b] = Some x.`3 
+                                     /\ (x.`1, x.`2, b, x.`4, x.`5) \notin Name_Red.O_UAKE_RN.unreg_ro{2}))
+               /\ (forall x, x \in UAKEc.HROc.RO.m{1} => (x.`4 \in Name_Red.O_UAKE_RN.x_set{2} \/ x.`4 \in Name_Red.O_UAKE_RN.pk_set{2}) 
+                                     /\ (x.`5 \in Name_Red.O_UAKE_RN.y_set{2} \/ x.`5 \in Name_Red.O_UAKE_RN.pk_set{2}))
+               /\ (forall x, x \in UAKE_mod.HROc.RO.m{2} => (x.`4 \in Name_Red.O_UAKE_RN.x_set{2} \/ x.`4 \in Name_Red.O_UAKE_RN.pk_set{2}) 
+                                     /\ (x.`5 \in Name_Red.O_UAKE_RN.y_set{2} \/ x.`5 \in Name_Red.O_UAKE_RN.pk_set{2}))
+               /\ (forall x, x \in Name_Red.O_UAKE_RN.unreg_ro{2} => x.`4 \in Name_Red.O_UAKE_RN.x_set{2} /\ x.`5 \in Name_Red.O_UAKE_RN.y_set{2})
 
-               /\ (forall i, omap rem_sid_c GAKEb_st.c_smap{1}.[i] = GAKE_mod.GAKEb_nodhs.c_smap{2}.[i])
-               /\ (forall i b pk m3, i \in GAKEb_st.c_smap{1} => get_trace (oget GAKEb_st.c_smap{1}.[i]) = Some ((b, pk), m3)
-                   => b \in Name_Red.O_GAKE.sid_pk{2}
-                                     /\ get_trace (rem_sid_c (oget GAKEb_st.c_smap{1}.[i])) 
-                                         = Some ((oget Name_Red.O_GAKE.sid_pk{2}.[b], pk), m3))                  
-               /\ (forall i pk_s pk m3, i \in GAKE_mod.GAKEb_nodhs.c_smap{2} => get_trace (oget GAKE_mod.GAKEb_nodhs.c_smap{2}.[i]) = Some ((pk_s, pk), m3)
-                    => pk_s \in Name_Red.O_GAKE.pk_set{2})
-               /\ (forall i pk_s b pk m3, i \in GAKE_mod.GAKEb_nodhs.c_smap{2} => get_trace (rem_sid_c (oget GAKEb_st.c_smap{1}.[i])) = Some ((pk_s, pk), m3)
-                    => b \in Name_Red.O_GAKE.sid_pk{2} => pk_s = oget Name_Red.O_GAKE.sid_pk{2}.[b]
-                    => get_trace (oget GAKEb_st.c_smap{1}.[i]) = Some ((b, pk), m3))  
-               /\ (forall i st pt ir x1 x2 x5, i \in GAKEb_st.c_smap{1} => GAKEb_st.c_smap{1}.[i] = Some (Pending st pt ir) 
-                    => st.`1 \in GAKEb_st.servers{1} /\ get_pkey (oget GAKEb_st.servers{1}.[st.`1]) = st.`2
+               /\ (forall i, omap rem_sid_c UAKE_name_st.c_smap{1}.[i] = UAKE_mod.O_RPK.c_smap{2}.[i])
+               /\ (forall i b pk m3, i \in UAKE_name_st.c_smap{1} => get_trace (oget UAKE_name_st.c_smap{1}.[i]) = Some ((b, pk), m3)
+                   => b \in Name_Red.O_UAKE_RN.sid_pk{2}
+                                     /\ get_trace (rem_sid_c (oget UAKE_name_st.c_smap{1}.[i])) 
+                                         = Some ((oget Name_Red.O_UAKE_RN.sid_pk{2}.[b], pk), m3))                  
+               /\ (forall i pk_s pk m3, i \in UAKE_mod.O_RPK.c_smap{2} => get_trace (oget UAKE_mod.O_RPK.c_smap{2}.[i]) = Some ((pk_s, pk), m3)
+                    => pk_s \in Name_Red.O_UAKE_RN.pk_set{2})
+               /\ (forall i pk_s b pk m3, i \in UAKE_mod.O_RPK.c_smap{2} => get_trace (rem_sid_c (oget UAKE_name_st.c_smap{1}.[i])) = Some ((pk_s, pk), m3)
+                    => b \in Name_Red.O_UAKE_RN.sid_pk{2} => pk_s = oget Name_Red.O_UAKE_RN.sid_pk{2}.[b]
+                    => get_trace (oget UAKE_name_st.c_smap{1}.[i]) = Some ((b, pk), m3))  
+               /\ (forall i st pt ir x1 x2 x5, i \in UAKE_name_st.c_smap{1} => UAKE_name_st.c_smap{1}.[i] = Some (Pending st pt ir) 
+                    => st.`1 \in UAKE_name_st.servers{1} /\ get_pkey (oget UAKE_name_st.servers{1}.[st.`1]) = st.`2
                                      /\ st.`1 = pt.`1
-                                     /\ g ^ st.`3 \in Name_Red.O_GAKE.pk_set{2} 
-                                     /\ (x1, x2, st.`1, g ^ st.`3, x5) \notin GAKEb_st.unreg_ro{1})
-               /\ (forall i st t k ir, i \in GAKEb_st.c_smap{1} => GAKEb_st.c_smap{1}.[i] = Some (Accepted st t k ir)
-                    => st.`1 \in Name_Red.O_GAKE.sid_pk{2} /\ (oget Name_Red.O_GAKE.sid_pk{2}.[st.`1]) = st.`2 /\ st.`1 = t.`1.`1 /\ t.`2 <> None)
+                                     /\ g ^ st.`3 \in Name_Red.O_UAKE_RN.pk_set{2} 
+                                     /\ (x1, x2, st.`1, g ^ st.`3, x5) \notin UAKE_name_st.unreg_ro{1})
+               /\ (forall i st t k ir, i \in UAKE_name_st.c_smap{1} => UAKE_name_st.c_smap{1}.[i] = Some (Accepted st t k ir)
+                    => st.`1 \in Name_Red.O_UAKE_RN.sid_pk{2} /\ (oget Name_Red.O_UAKE_RN.sid_pk{2}.[st.`1]) = st.`2 /\ st.`1 = t.`1.`1 /\ t.`2 <> None)
 
-               /\ (forall b j, (b, j) \in GAKEb_st.s_smap{1} => b \in Name_Red.O_GAKE.sid_pk{2}
-                                     /\ ((oget Name_Red.O_GAKE.sid_pk{2}.[b]), j) \in GAKE_mod.GAKEb_nodhs.s_smap{2}
-                                     /\ rem_sid_s (oget GAKEb_st.s_smap{1}.[(b, j)]) = oget GAKE_mod.GAKEb_nodhs.s_smap{2}.[(oget Name_Red.O_GAKE.sid_pk{2}.[b]), j])
-               /\ (forall b j, b \in Name_Red.O_GAKE.sid_pk{2}
-                    => (oget Name_Red.O_GAKE.sid_pk{2}.[b], j) \in GAKE_mod.GAKEb_nodhs.s_smap{2} <=> (b, j) \in GAKEb_st.s_smap{1})
-               /\ (forall b j st t k ir, (b, j) \in GAKEb_st.s_smap{1} => GAKEb_st.s_smap{1}.[(b, j)] = Some (Accepted st t k ir)
-                    => t.`1.`1 = b /\ t.`2 <> None /\ Name_Red.O_GAKE.sid_pk{2}.[b] = Some (g ^ st.`2))
-               /\ (forall pk j st t k ir, (pk, j) \in GAKE_mod.GAKEb_nodhs.s_smap{2} => GAKE_mod.GAKEb_nodhs.s_smap{2}.[(pk, j)] = Some (Accepted_mod st t k ir)
+               /\ (forall b j, (b, j) \in UAKE_name_st.s_smap{1} => b \in Name_Red.O_UAKE_RN.sid_pk{2}
+                                     /\ ((oget Name_Red.O_UAKE_RN.sid_pk{2}.[b]), j) \in UAKE_mod.O_RPK.s_smap{2}
+                                     /\ rem_sid_s (oget UAKE_name_st.s_smap{1}.[(b, j)]) = oget UAKE_mod.O_RPK.s_smap{2}.[(oget Name_Red.O_UAKE_RN.sid_pk{2}.[b]), j])
+               /\ (forall b j, b \in Name_Red.O_UAKE_RN.sid_pk{2}
+                    => (oget Name_Red.O_UAKE_RN.sid_pk{2}.[b], j) \in UAKE_mod.O_RPK.s_smap{2} <=> (b, j) \in UAKE_name_st.s_smap{1})
+               /\ (forall b j st t k ir, (b, j) \in UAKE_name_st.s_smap{1} => UAKE_name_st.s_smap{1}.[(b, j)] = Some (Accepted st t k ir)
+                    => t.`1.`1 = b /\ t.`2 <> None /\ Name_Red.O_UAKE_RN.sid_pk{2}.[b] = Some (g ^ st.`2))
+               /\ (forall pk j st t k ir, (pk, j) \in UAKE_mod.O_RPK.s_smap{2} => UAKE_mod.O_RPK.s_smap{2}.[(pk, j)] = Some (Accepted_mod st t k ir)
                     => t.`1.`1 = pk)
-               /\ (forall pk_s j, (pk_s, j) \in GAKE_mod.GAKEb_nodhs.s_smap{2} => (exists pk m3, get_trace (oget GAKE_mod.GAKEb_nodhs.s_smap{2}.[pk_s, j]) = Some ((pk_s, pk), m3)))
-               /\ (forall bj pk m3, bj \in GAKEb_st.s_smap{1} => get_trace (oget GAKEb_st.s_smap{1}.[bj]) = Some ((bj.`1, pk), m3)
-                    => bj.`1 \in Name_Red.O_GAKE.sid_pk{2}
-                                     /\ get_trace (rem_sid_s (oget GAKEb_st.s_smap{1}.[bj])) 
-                                         = Some ((oget Name_Red.O_GAKE.sid_pk{2}.[bj.`1], pk), m3))
-               /\ (forall b j pk_s pk m3, (pk_s, j) \in GAKE_mod.GAKEb_nodhs.s_smap{2} => get_trace (oget GAKE_mod.GAKEb_nodhs.s_smap{2}.[(pk_s,j)]) = Some ((pk_s, pk), m3)
-                    => b \in Name_Red.O_GAKE.sid_pk{2} => pk_s = oget Name_Red.O_GAKE.sid_pk{2}.[b]
-                    => get_trace (oget GAKEb_st.s_smap{1}.[(b, j)]) = Some ((b, pk), m3))
+               /\ (forall pk_s j, (pk_s, j) \in UAKE_mod.O_RPK.s_smap{2} => (exists pk m3, get_trace (oget UAKE_mod.O_RPK.s_smap{2}.[pk_s, j]) = Some ((pk_s, pk), m3)))
+               /\ (forall bj pk m3, bj \in UAKE_name_st.s_smap{1} => get_trace (oget UAKE_name_st.s_smap{1}.[bj]) = Some ((bj.`1, pk), m3)
+                    => bj.`1 \in Name_Red.O_UAKE_RN.sid_pk{2}
+                                     /\ get_trace (rem_sid_s (oget UAKE_name_st.s_smap{1}.[bj])) 
+                                         = Some ((oget Name_Red.O_UAKE_RN.sid_pk{2}.[bj.`1], pk), m3))
+               /\ (forall b j pk_s pk m3, (pk_s, j) \in UAKE_mod.O_RPK.s_smap{2} => get_trace (oget UAKE_mod.O_RPK.s_smap{2}.[(pk_s,j)]) = Some ((pk_s, pk), m3)
+                    => b \in Name_Red.O_UAKE_RN.sid_pk{2} => pk_s = oget Name_Red.O_UAKE_RN.sid_pk{2}.[b]
+                    => get_trace (oget UAKE_name_st.s_smap{1}.[(b, j)]) = Some ((b, pk), m3))
 
-               /\ (forall b, b \in GAKEb_st.servers{1} <=> b \in Name_Red.O_GAKE.sid_pk{2})
-               /\ (forall b, b \in GAKEb_st.servers{1} => get_pkey (oget GAKEb_st.servers{1}.[b]) = (oget Name_Red.O_GAKE.sid_pk{2}.[b])
-                                     /\ !get_sr_dh (oget GAKEb_st.servers{1}.[b])
-                                     /\ get_pkey (oget GAKEb_st.servers{1}.[b]) \in GAKE_mod.GAKEb_nodhs.servers{2}
-                                     /\ (get_sr_ltk (oget GAKEb_st.servers{1}.[b]) 
-                                         <=> get_sr_ltk (oget GAKE_mod.GAKEb_nodhs.servers{2}.[oget Name_Red.O_GAKE.sid_pk{2}.[b]])))
-               /\ (forall pk b sk1 sk2, pk \in GAKE_mod.GAKEb_nodhs.servers{2} => obind GAKE_mod.get_skey GAKE_mod.GAKEb_nodhs.servers{2}.[pk] = Some sk1 
-                    => b \in GAKEb_st.servers{1} => obind GAKEc.get_skey GAKEb_st.servers{1}.[b] = Some sk2 
-                    => b \in Name_Red.O_GAKE.sid_pk{2} => (oget Name_Red.O_GAKE.sid_pk{2}.[b]) = pk => sk1 = sk2)
-               /\ (forall b, b \in Name_Red.O_GAKE.sid_pk{2} => (oget Name_Red.O_GAKE.sid_pk{2}.[b]) \in Name_Red.O_GAKE.pk_set{2})
-               /\ (forall b pk, b \in Name_Red.O_GAKE.sid_pk{2} => oget Name_Red.O_GAKE.sid_pk{2}.[b] = pk
-                    =>  obind GAKE_mod.get_skey GAKE_mod.GAKEb_nodhs.servers{2}.[pk] <> None)
-               /\ (forall sk, g ^ sk \in GAKE_mod.GAKEb_nodhs.servers{2} => obind GAKE_mod.get_skey GAKE_mod.GAKEb_nodhs.servers{2}.[g ^ sk] = Some sk)
-               /\ (forall sk pk b, b \in Name_Red.O_GAKE.sid_pk{2} => oget Name_Red.O_GAKE.sid_pk{2}.[b] = pk
-                    => pk \in GAKE_mod.GAKEb_nodhs.servers{2} => obind GAKE_mod.get_skey GAKE_mod.GAKEb_nodhs.servers{2}.[pk] = Some sk 
+               /\ (forall b, b \in UAKE_name_st.servers{1} <=> b \in Name_Red.O_UAKE_RN.sid_pk{2})
+               /\ (forall b, b \in UAKE_name_st.servers{1} => get_pkey (oget UAKE_name_st.servers{1}.[b]) = (oget Name_Red.O_UAKE_RN.sid_pk{2}.[b])
+                                     /\ !get_sr_dh (oget UAKE_name_st.servers{1}.[b])
+                                     /\ get_pkey (oget UAKE_name_st.servers{1}.[b]) \in UAKE_mod.O_RPK.servers{2}
+                                     /\ (get_sr_ltk (oget UAKE_name_st.servers{1}.[b]) 
+                                         <=> get_sr_ltk (oget UAKE_mod.O_RPK.servers{2}.[oget Name_Red.O_UAKE_RN.sid_pk{2}.[b]])))
+               /\ (forall pk b sk1 sk2, pk \in UAKE_mod.O_RPK.servers{2} => obind UAKE_mod.get_skey UAKE_mod.O_RPK.servers{2}.[pk] = Some sk1 
+                    => b \in UAKE_name_st.servers{1} => obind UAKEc.get_skey UAKE_name_st.servers{1}.[b] = Some sk2 
+                    => b \in Name_Red.O_UAKE_RN.sid_pk{2} => (oget Name_Red.O_UAKE_RN.sid_pk{2}.[b]) = pk => sk1 = sk2)
+               /\ (forall b, b \in Name_Red.O_UAKE_RN.sid_pk{2} => (oget Name_Red.O_UAKE_RN.sid_pk{2}.[b]) \in Name_Red.O_UAKE_RN.pk_set{2})
+               /\ (forall b pk, b \in Name_Red.O_UAKE_RN.sid_pk{2} => oget Name_Red.O_UAKE_RN.sid_pk{2}.[b] = pk
+                    =>  obind UAKE_mod.get_skey UAKE_mod.O_RPK.servers{2}.[pk] <> None)
+               /\ (forall sk, g ^ sk \in UAKE_mod.O_RPK.servers{2} => obind UAKE_mod.get_skey UAKE_mod.O_RPK.servers{2}.[g ^ sk] = Some sk)
+               /\ (forall sk pk b, b \in Name_Red.O_UAKE_RN.sid_pk{2} => oget Name_Red.O_UAKE_RN.sid_pk{2}.[b] = pk
+                    => pk \in UAKE_mod.O_RPK.servers{2} => obind UAKE_mod.get_skey UAKE_mod.O_RPK.servers{2}.[pk] = Some sk 
                     => pk = g ^ sk)
-               /\ (forall pk j x1 x2 x4 x5, pk \notin Name_Red.O_GAKE.pk_set{2} 
-                    => pk \notin GAKE_mod.GAKEb_nodhs.servers{2} /\ (pk, j) \notin GAKE_mod.GAKEb_nodhs.s_smap{2} /\ (x1, x2, pk, x4, x5) \notin GAKE_mod.HROc.RO.m{2})
-               /\ (forall b1 b2, b1 \in Name_Red.O_GAKE.sid_pk{2} => b2 \in Name_Red.O_GAKE.sid_pk{2} 
-                    => (oget Name_Red.O_GAKE.sid_pk{2}.[b1]) = (oget Name_Red.O_GAKE.sid_pk{2}.[b2])
+               /\ (forall pk j x1 x2 x4 x5, pk \notin Name_Red.O_UAKE_RN.pk_set{2} 
+                    => pk \notin UAKE_mod.O_RPK.servers{2} /\ (pk, j) \notin UAKE_mod.O_RPK.s_smap{2} /\ (x1, x2, pk, x4, x5) \notin UAKE_mod.HROc.RO.m{2})
+               /\ (forall b1 b2, b1 \in Name_Red.O_UAKE_RN.sid_pk{2} => b2 \in Name_Red.O_UAKE_RN.sid_pk{2} 
+                    => (oget Name_Red.O_UAKE_RN.sid_pk{2}.[b1]) = (oget Name_Red.O_UAKE_RN.sid_pk{2}.[b2])
                     => b1 = b2)
-          , (GAKEb_st.stop1{1} \/ GAKEb_st.stop2{1}) = (Name_Red.O_GAKE.stop1{2} \/ Name_Red.O_GAKE.stop2{2})) => //; last first.
+          , (UAKE_name_st.stop1{1} \/ UAKE_name_st.stop2{1}) = (Name_Red.O_UAKE_RN.stop1{2} \/ Name_Red.O_UAKE_RN.stop2{2})) => //; last first.
 auto => />.
 split. smt(emptyE in_fset0).
 move => 50? st1r st2r 8?.
@@ -2332,7 +2327,7 @@ case : (!(st1r \/ st2r)) => />. smt().
         move => i1 b1 pk0 m3 iin.
         case (b{2} = b1) => beq; 2: by smt(get_setE mem_set in_fsetU1).
         rewrite beq get_setE //=.
-        have<-: oget GAKE_mod.GAKEb_nodhs.c_smap{2}.[i1] = rem_sid_c (oget GAKEb_st.c_smap{1}.[i1]). smt().
+        have<-: oget UAKE_mod.O_RPK.c_smap{2}.[i1] = rem_sid_c (oget UAKE_name_st.c_smap{1}.[i1]). smt().
         smt(get_setE mem_set in_fsetU1).
       match None {2} ^match. auto => />.
       auto => /> &1 &2 *. smt(get_setE mem_set in_fsetU1).
@@ -2348,7 +2343,7 @@ case : (!(st1r \/ st2r)) => />. smt().
   rcondf ^if; auto => />.
 
 - proc; inline.
-  case (Name_Red.O_GAKE.stop1{2} \/ Name_Red.O_GAKE.stop2{2}).
+  case (Name_Red.O_UAKE_RN.stop1{2} \/ Name_Red.O_UAKE_RN.stop2{2}).
   + rcondf {2} ^if. auto => />.
     sp; if {1} => //.
     + sp; match {1} => //. 
@@ -2377,7 +2372,7 @@ case : (!(st1r \/ st2r)) => />. smt().
   auto => />.
 
 - proc; inline. 
-  case (Name_Red.O_GAKE.stop1{2} \/ Name_Red.O_GAKE.stop2{2}).
+  case (Name_Red.O_UAKE_RN.stop1{2} \/ Name_Red.O_UAKE_RN.stop2{2}).
   + rcondf {2} ^if. auto => />.
     sp; match {1} => //. 
     + auto => />.
@@ -2465,13 +2460,13 @@ case : (!(st1r \/ st2r)) => />. smt().
         rewrite !get_setE ieq //=.
         rewrite /rem_sid_c //=.
         do split; ~4: smt(get_setE mem_set in_fsetU1 pow_bij).
-        have : Name_Red.O_GAKE.sid_pk{2}.[b{1}] = Some pk_b{2} by smt(get_setE mem_set in_fsetU1 pow_bij).
+        have : Name_Red.O_UAKE_RN.sid_pk{2}.[b{1}] = Some pk_b{2} by smt(get_setE mem_set in_fsetU1 pow_bij).
         move => bpk.
         have : (t_A{2}, sk{2}) = (m3{2}.`2, sk{1}).
         + have := inv (m3{2}.`1 ^ sk_ce{1}, pk_b{1} ^ sk_ce{1}, b{1}, g ^ sk_ce{1}, m3{2}.`1). 
           have->: (m3{2}.`1 ^ sk_ce{1}, pk_b{1} ^ sk_ce{1}, b{1}, g ^ sk_ce{1}, m3{2}.`1) \in HROc.RO.m{1} by smt().
-          have->:  b{1} \in Name_Red.O_GAKE.sid_pk{2} by smt().
-          have->:  (m3{2}.`1 ^ sk_ce{1}, pk_b{1} ^ sk_ce{1}, b{1}, g ^ sk_ce{1}, m3{2}.`1) \notin Name_Red.O_GAKE.unreg_ro{2} by smt().
+          have->:  b{1} \in Name_Red.O_UAKE_RN.sid_pk{2} by smt().
+          have->:  (m3{2}.`1 ^ sk_ce{1}, pk_b{1} ^ sk_ce{1}, b{1}, g ^ sk_ce{1}, m3{2}.`1) \notin Name_Red.O_UAKE_RN.unreg_ro{2} by smt().
           rewrite roxl roxr.
           smt(get_setE mem_set in_fsetU1 pow_bij). 
         smt().
@@ -2481,13 +2476,13 @@ case : (!(st1r \/ st2r)) => />. smt().
       rewrite !get_setE ieq //=.
       rewrite /rem_sid_c //=.
       do split; ~4: smt(get_setE mem_set in_fsetU1 pow_bij).
-      have : Name_Red.O_GAKE.sid_pk{2}.[b{1}] = Some pk_b{2} by smt(get_setE mem_set in_fsetU1 pow_bij).
+      have : Name_Red.O_UAKE_RN.sid_pk{2}.[b{1}] = Some pk_b{2} by smt(get_setE mem_set in_fsetU1 pow_bij).
       move => bpk.
       have : (t_A{2}, sk{2}) = (m3{2}.`2, sk{1}).
       + have := inv (m3{2}.`1 ^ sk_ce{1}, pk_b{1} ^ sk_ce{1}, b{1}, g ^ sk_ce{1}, m3{2}.`1). 
         have-> : (m3{2}.`1 ^ sk_ce{1}, pk_b{1} ^ sk_ce{1}, b{1}, g ^ sk_ce{1}, m3{2}.`1) \in HROc.RO.m{1} by smt().
-        have-> :  b{1} \in Name_Red.O_GAKE.sid_pk{2} by smt().
-        have-> :  (m3{2}.`1 ^ sk_ce{1}, pk_b{1} ^ sk_ce{1}, b{1}, g ^ sk_ce{1}, m3{2}.`1) \notin Name_Red.O_GAKE.unreg_ro{2} by smt().
+        have-> :  b{1} \in Name_Red.O_UAKE_RN.sid_pk{2} by smt().
+        have-> :  (m3{2}.`1 ^ sk_ce{1}, pk_b{1} ^ sk_ce{1}, b{1}, g ^ sk_ce{1}, m3{2}.`1) \notin Name_Red.O_UAKE_RN.unreg_ro{2} by smt().
         rewrite roxl roxr.
         smt(get_setE mem_set in_fsetU1 pow_bij). 
       smt().
@@ -2518,9 +2513,9 @@ case : (!(st1r \/ st2r)) => />. smt().
     if => //.
     + auto => /> &1 &2 25? inv inv2 *. 
       rewrite /untested_partner_c. 
-      have<-: (card (get_partners_c t'{1} GAKEb_st.s_smap{1}) = card (get_partners_c t'{2} GAKE_mod.GAKEb_nodhs.s_smap{2})).
+      have<-: (card (get_partners_c t'{1} UAKE_name_st.s_smap{1}) = card (get_partners_c t'{2} UAKE_mod.O_RPK.s_smap{2})).
       + rewrite /get_partners_c.
-        rewrite -(inj_fcard_image_pw (fun (bj : s_id * int) => (oget Name_Red.O_GAKE.sid_pk{2}.[bj.`1], bj.`2))).
+        rewrite -(inj_fcard_image_pw (fun (bj : s_id * int) => (oget Name_Red.O_UAKE_RN.sid_pk{2}.[bj.`1], bj.`2))).
         + move => x y.
           rewrite !mem_fdom !mem_filter //=.
           smt(get_setE mem_set in_fsetU1 pow_bij).
@@ -2534,7 +2529,7 @@ case : (!(st1r \/ st2r)) => />. smt().
           rewrite !mem_fdom !mem_filter //=.
           move => [] ain tra ax.
           split; 1: smt(get_setE mem_set).
-          have->: oget GAKE_mod.GAKEb_nodhs.s_smap{2}.[x] = rem_sid_s (oget GAKEb_st.s_smap{1}.[a]). smt().
+          have->: oget UAKE_mod.O_RPK.s_smap{2}.[x] = rem_sid_s (oget UAKE_name_st.s_smap{1}.[a]). smt().
           have : (Accepted_mod st'{2} t'{2} k'{2} ir'{2}) = rem_sid_c (Accepted st'{1} t'{1} k'{1} ir'{1}). smt().
           rewrite /rem_sid_c //=.
           move => [#] steq teq keq ireq.
@@ -2551,14 +2546,14 @@ case : (!(st1r \/ st2r)) => />. smt().
         have : st'{1}.`2 = x.`1 by smt(get_setE mem_set in_fsetU1 pow_bij).
         move => x1eq.
         split. split.
-        + have : t'{1}.`1.`1 \in Name_Red.O_GAKE.sid_pk{2} by smt().
+        + have : t'{1}.`1.`1 \in Name_Red.O_UAKE_RN.sid_pk{2} by smt().
           smt(get_setE mem_set).
         + have v := inv2 t'{1}.`1.`1 x.`2 st'{1}.`2 t'{1}.`1.`2 t'{1}.`2.
           by rewrite v; smt().
         smt(get_setE mem_set in_fsetU1 pow_bij).
-      have<-: (card (get_untested_partners_c t'{1} GAKEb_st.s_smap{1}) = card (get_untested_partners_c t'{2} GAKE_mod.GAKEb_nodhs.s_smap{2})).
+      have<-: (card (get_untested_partners_c t'{1} UAKE_name_st.s_smap{1}) = card (get_untested_partners_c t'{2} UAKE_mod.O_RPK.s_smap{2})).
       + rewrite /get_untested_partners_c.
-        rewrite -(inj_fcard_image_pw (fun (bj : s_id * int) => (oget Name_Red.O_GAKE.sid_pk{2}.[bj.`1], bj.`2))).
+        rewrite -(inj_fcard_image_pw (fun (bj : s_id * int) => (oget Name_Red.O_UAKE_RN.sid_pk{2}.[bj.`1], bj.`2))).
         + move => x y.
           rewrite !mem_fdom !mem_filter //=.
           smt(get_setE mem_set in_fsetU1 pow_bij).
@@ -2572,7 +2567,7 @@ case : (!(st1r \/ st2r)) => />. smt().
           rewrite !mem_fdom !mem_filter //=.
           move => [] ain tra ax.
           split; 1: smt(get_setE mem_set).
-          have->: oget GAKE_mod.GAKEb_nodhs.s_smap{2}.[x] = rem_sid_s (oget GAKEb_st.s_smap{1}.[a]) by smt().
+          have->: oget UAKE_mod.O_RPK.s_smap{2}.[x] = rem_sid_s (oget UAKE_name_st.s_smap{1}.[a]) by smt().
           have : (Accepted_mod st'{2} t'{2} k'{2} ir'{2}) = rem_sid_c (Accepted st'{1} t'{1} k'{1} ir'{1}) by smt().
           rewrite /rem_sid_c //=.
           move => [#] steq teq keq ireq.
@@ -2589,7 +2584,7 @@ case : (!(st1r \/ st2r)) => />. smt().
         have : st'{1}.`2 = x.`1 by smt(get_setE mem_set in_fsetU1 pow_bij).
         move => x1eq.
         split. split.
-        + have : t'{1}.`1.`1 \in Name_Red.O_GAKE.sid_pk{2} by smt().
+        + have : t'{1}.`1.`1 \in Name_Red.O_UAKE_RN.sid_pk{2} by smt().
           smt(get_setE mem_set).
         + have v := inv2 t'{1}.`1.`1 x.`2 st'{1}.`2 t'{1}.`1.`2 t'{1}.`2.
           rewrite v; smt().
@@ -2622,16 +2617,16 @@ case : (!(st1r \/ st2r)) => />. smt().
     + auto => /> &1 &2 14? inv3 inv ? inv2 *.
       rewrite /untested_partner_s.
       rewrite /get_partners_s.
-      have-> : (fdom (filter (fun (_ : int) (val : GAKEc.pr_st_client GAKEc.instance_state) => get_trace val 
-                 = Some t'{1}) GAKEb_st.c_smap{1})) = (fdom (filter (fun (_ : int)
-              (val : GAKE_mod.pr_st_client GAKE_mod.instance_state) => get_trace val = Some t'{2}) GAKE_mod.GAKEb_nodhs.c_smap{2})).
+      have-> : (fdom (filter (fun (_ : int) (val : UAKEc.c_state UAKEc.instance_state) => get_trace val 
+                 = Some t'{1}) UAKE_name_st.c_smap{1})) = (fdom (filter (fun (_ : int)
+              (val : UAKE_mod.c_state UAKE_mod.instance_state) => get_trace val = Some t'{2}) UAKE_mod.O_RPK.c_smap{2})).
       + rewrite fsetP.
         move => x.
         rewrite !mem_fdom !mem_filter //=.
         split. 
         + move => [] xin trx.
           split; 1: smt(get_setE mem_set in_fsetU1 pow_bij).
-          have->: oget GAKE_mod.GAKEb_nodhs.c_smap{2}.[x] = rem_sid_c (oget GAKEb_st.c_smap{1}.[x]) by smt().
+          have->: oget UAKE_mod.O_RPK.c_smap{2}.[x] = rem_sid_c (oget UAKE_name_st.c_smap{1}.[x]) by smt().
           have : (Accepted_mod st'{2} t'{2} k'{2} ir'{2}) = rem_sid_s (Accepted st'{1} t'{1} k'{1} ir'{1}) by smt().
           rewrite /rem_sid_s //=.
           move => [#] steq teq keq ireq.
@@ -2640,17 +2635,17 @@ case : (!(st1r \/ st2r)) => />. smt().
           smt().
         smt(get_setE mem_set in_fsetU1 pow_bij).
       rewrite /get_untested_partners_s.
-      have->: (fdom (filter (fun (_ : int) (val : GAKEc.pr_st_client GAKEc.instance_state) =>
-                  get_trace val = Some t'{1} /\ get_ir_test val = false) GAKEb_st.c_smap{1})) = (fdom
-                (filter (fun (_ : int) (val : GAKE_mod.pr_st_client GAKE_mod.instance_state) =>
-                  get_trace val = Some t'{2} /\ get_ir_test val = false) GAKE_mod.GAKEb_nodhs.c_smap{2})).
+      have->: (fdom (filter (fun (_ : int) (val : UAKEc.c_state UAKEc.instance_state) =>
+                  get_trace val = Some t'{1} /\ get_ir_test val = false) UAKE_name_st.c_smap{1})) = (fdom
+                (filter (fun (_ : int) (val : UAKE_mod.c_state UAKE_mod.instance_state) =>
+                  get_trace val = Some t'{2} /\ get_ir_test val = false) UAKE_mod.O_RPK.c_smap{2})).
       + rewrite fsetP.
         move => x.
         rewrite !mem_fdom !mem_filter //=.
         split. 
         + move => [] xin [] trx xnt.
           split; 1: smt(get_setE mem_set in_fsetU1 pow_bij).
-          have->: oget GAKE_mod.GAKEb_nodhs.c_smap{2}.[x] = rem_sid_c (oget GAKEb_st.c_smap{1}.[x]) by smt().
+          have->: oget UAKE_mod.O_RPK.c_smap{2}.[x] = rem_sid_c (oget UAKE_name_st.c_smap{1}.[x]) by smt().
           have : (Accepted_mod st'{2} t'{2} k'{2} ir'{2}) = rem_sid_s (Accepted st'{1} t'{1} k'{1} ir'{1}) by smt().
           rewrite /rem_sid_s //=.
           move => [#] steq teq keq ireq.
@@ -2667,7 +2662,7 @@ case : (!(st1r \/ st2r)) => />. smt().
         move => [#] steq teq keq ireq.
         rewrite teq.
         move => [] xin.
-        have->: oget GAKE_mod.GAKEb_nodhs.c_smap{2}.[x] = rem_sid_c (oget GAKEb_st.c_smap{1}.[x]) by smt().
+        have->: oget UAKE_mod.O_RPK.c_smap{2}.[x] = rem_sid_c (oget UAKE_name_st.c_smap{1}.[x]) by smt().
         move => trx.
         have v := inv2 x (g ^ st'{1}.`2) b{2} t'{1}.`1.`2 t'{1}.`2.
         rewrite v; 1..4: smt(). 
@@ -2701,66 +2696,66 @@ case : (!(st1r \/ st2r)) => />. smt().
       + auto => /> &1 &2 15? inv ? inv2 *.
         split.
         + move => + j pkin - /(_ j).
-          have : (b{2}, j) \in GAKEb_st.s_smap{1} by smt().
+          have : (b{2}, j) \in UAKE_name_st.s_smap{1} by smt().
           move => bjin //=.
           rewrite /untested_partner_s.
           rewrite /get_partners_s /get_untested_partners_s.
-          have->: (fdom (filter (fun (_ : int) (val : GAKE_mod.pr_st_client GAKE_mod.instance_state) => get_trace val =
-                     Some (oget (get_trace (oget GAKE_mod.GAKEb_nodhs.s_smap{2}.[oget Name_Red.O_GAKE.sid_pk{2}.[b{2}], j]))))
-                   GAKE_mod.GAKEb_nodhs.c_smap{2})) = (fdom (filter (fun (_ : int) (val : GAKEc.pr_st_client GAKEc.instance_state) =>
-                     get_trace val = Some (oget (get_trace (oget GAKEb_st.s_smap{1}.[b{2}, j])))) GAKEb_st.c_smap{1})).
+          have->: (fdom (filter (fun (_ : int) (val : UAKE_mod.c_state UAKE_mod.instance_state) => get_trace val =
+                     Some (oget (get_trace (oget UAKE_mod.O_RPK.s_smap{2}.[oget Name_Red.O_UAKE_RN.sid_pk{2}.[b{2}], j]))))
+                   UAKE_mod.O_RPK.c_smap{2})) = (fdom (filter (fun (_ : int) (val : UAKEc.c_state UAKEc.instance_state) =>
+                     get_trace val = Some (oget (get_trace (oget UAKE_name_st.s_smap{1}.[b{2}, j])))) UAKE_name_st.c_smap{1})).
           + rewrite fsetP.
             move => x.
             rewrite !mem_fdom !mem_filter //=.
             smt().
-          have->: (fdom (filter (fun (_ : int) (val : GAKE_mod.pr_st_client GAKE_mod.instance_state) => get_trace val =
-                     Some (oget (get_trace (oget GAKE_mod.GAKEb_nodhs.s_smap{2}.[oget Name_Red.O_GAKE.sid_pk{2}.[b{2}], j]))) /\
-                   get_ir_test val = false) GAKE_mod.GAKEb_nodhs.c_smap{2})) = (fdom (filter (fun (_ : int)
-                     (val : GAKEc.pr_st_client GAKEc.instance_state) => get_trace val = Some (oget (get_trace
-                   (oget GAKEb_st.s_smap{1}.[b{2}, j]))) /\ get_ir_test val = false) GAKEb_st.c_smap{1})).
+          have->: (fdom (filter (fun (_ : int) (val : UAKE_mod.c_state UAKE_mod.instance_state) => get_trace val =
+                     Some (oget (get_trace (oget UAKE_mod.O_RPK.s_smap{2}.[oget Name_Red.O_UAKE_RN.sid_pk{2}.[b{2}], j]))) /\
+                   get_ir_test val = false) UAKE_mod.O_RPK.c_smap{2})) = (fdom (filter (fun (_ : int)
+                     (val : UAKEc.c_state UAKEc.instance_state) => get_trace val = Some (oget (get_trace
+                   (oget UAKE_name_st.s_smap{1}.[b{2}, j]))) /\ get_ir_test val = false) UAKE_name_st.c_smap{1})).
           + rewrite fsetP.
             move => x.
             rewrite !mem_fdom !mem_filter //=.
             split.
             + move => [#] xin trx.
-              have->: oget GAKE_mod.GAKEb_nodhs.c_smap{2}.[x] = rem_sid_c (oget GAKEb_st.c_smap{1}.[x]). smt().
+              have->: oget UAKE_mod.O_RPK.c_smap{2}.[x] = rem_sid_c (oget UAKE_name_st.c_smap{1}.[x]). smt().
               rewrite /rem_sid_c.
               move => xnt.
               do split; smt().
             move => [#] xin trx xnt.
-            have->: oget GAKE_mod.GAKEb_nodhs.c_smap{2}.[x] = rem_sid_c (oget GAKEb_st.c_smap{1}.[x]) by smt().
+            have->: oget UAKE_mod.O_RPK.c_smap{2}.[x] = rem_sid_c (oget UAKE_name_st.c_smap{1}.[x]) by smt().
             rewrite /rem_sid_c.
             do split; smt().
           smt().
         move => + j pkin - /(_ j).
-        have : (b{2}, j) \in GAKEb_st.s_smap{1} by smt().
+        have : (b{2}, j) \in UAKE_name_st.s_smap{1} by smt().
         move => bjin //=.
         rewrite /untested_partner_s.
         rewrite /get_partners_s /get_untested_partners_s.
-        have->: (fdom (filter (fun (_ : int) (val : GAKE_mod.pr_st_client GAKE_mod.instance_state) => get_trace val =
-                   Some (oget (get_trace (oget GAKE_mod.GAKEb_nodhs.s_smap{2}.[oget Name_Red.O_GAKE.sid_pk{2}.[b{2}], j]))))
-                 GAKE_mod.GAKEb_nodhs.c_smap{2})) = (fdom (filter (fun (_ : int) (val : GAKEc.pr_st_client GAKEc.instance_state) =>
-                   get_trace val = Some (oget (get_trace (oget GAKEb_st.s_smap{1}.[b{2}, j])))) GAKEb_st.c_smap{1})).
+        have->: (fdom (filter (fun (_ : int) (val : UAKE_mod.c_state UAKE_mod.instance_state) => get_trace val =
+                   Some (oget (get_trace (oget UAKE_mod.O_RPK.s_smap{2}.[oget Name_Red.O_UAKE_RN.sid_pk{2}.[b{2}], j]))))
+                 UAKE_mod.O_RPK.c_smap{2})) = (fdom (filter (fun (_ : int) (val : UAKEc.c_state UAKEc.instance_state) =>
+                   get_trace val = Some (oget (get_trace (oget UAKE_name_st.s_smap{1}.[b{2}, j])))) UAKE_name_st.c_smap{1})).
         + rewrite fsetP.
           move => x.
           rewrite !mem_fdom !mem_filter //=.
           smt().
-        have->: (fdom (filter (fun (_ : int) (val : GAKE_mod.pr_st_client GAKE_mod.instance_state) => get_trace val =
-                   Some (oget (get_trace (oget GAKE_mod.GAKEb_nodhs.s_smap{2}.[oget Name_Red.O_GAKE.sid_pk{2}.[b{2}], j]))) /\
-                 get_ir_test val = false) GAKE_mod.GAKEb_nodhs.c_smap{2})) = (fdom (filter (fun (_ : int)
-                   (val : GAKEc.pr_st_client GAKEc.instance_state) => get_trace val = Some (oget (get_trace
-                 (oget GAKEb_st.s_smap{1}.[b{2}, j]))) /\ get_ir_test val = false) GAKEb_st.c_smap{1})).
+        have->: (fdom (filter (fun (_ : int) (val : UAKE_mod.c_state UAKE_mod.instance_state) => get_trace val =
+                   Some (oget (get_trace (oget UAKE_mod.O_RPK.s_smap{2}.[oget Name_Red.O_UAKE_RN.sid_pk{2}.[b{2}], j]))) /\
+                 get_ir_test val = false) UAKE_mod.O_RPK.c_smap{2})) = (fdom (filter (fun (_ : int)
+                   (val : UAKEc.c_state UAKEc.instance_state) => get_trace val = Some (oget (get_trace
+                 (oget UAKE_name_st.s_smap{1}.[b{2}, j]))) /\ get_ir_test val = false) UAKE_name_st.c_smap{1})).
         + rewrite fsetP.
           move => x.
           rewrite !mem_fdom !mem_filter //=.
           split.
           + move => [#] xin trx.
-            have->: oget GAKE_mod.GAKEb_nodhs.c_smap{2}.[x] = rem_sid_c (oget GAKEb_st.c_smap{1}.[x]). smt().
+            have->: oget UAKE_mod.O_RPK.c_smap{2}.[x] = rem_sid_c (oget UAKE_name_st.c_smap{1}.[x]). smt().
             rewrite /rem_sid_c.
             move => xnt.
             do split; smt().
           move => [#] xin trx xnt.
-          have->: oget GAKE_mod.GAKEb_nodhs.c_smap{2}.[x] = rem_sid_c (oget GAKEb_st.c_smap{1}.[x]) by smt().
+          have->: oget UAKE_mod.O_RPK.c_smap{2}.[x] = rem_sid_c (oget UAKE_name_st.c_smap{1}.[x]) by smt().
           rewrite /rem_sid_c.
           do split; smt().
         smt().
@@ -2787,9 +2782,9 @@ case : (!(st1r \/ st2r)) => />. smt().
       if => //.
       + auto => /> &1 &2 25? inv inv2 *. 
         rewrite /tested_origins_c.
-        have<-: (card (get_origins_c (pk_e{1}, None) GAKEb_st.s_smap{1}) = card (get_origins_c (pk_e{2}, None) GAKE_mod.GAKEb_nodhs.s_smap{2})).
+        have<-: (card (get_origins_c (pk_e{1}, None) UAKE_name_st.s_smap{1}) = card (get_origins_c (pk_e{2}, None) UAKE_mod.O_RPK.s_smap{2})).
         + rewrite /get_origins_c. 
-          rewrite -(inj_fcard_image_pw (fun (bj : s_id * int) => (oget Name_Red.O_GAKE.sid_pk{2}.[bj.`1], bj.`2))).
+          rewrite -(inj_fcard_image_pw (fun (bj : s_id * int) => (oget Name_Red.O_UAKE_RN.sid_pk{2}.[bj.`1], bj.`2))).
           + move => x y.
             rewrite !mem_fdom !mem_filter //=.
             smt(get_setE mem_set in_fsetU1 pow_bij).
@@ -2803,7 +2798,7 @@ case : (!(st1r \/ st2r)) => />. smt().
             rewrite !mem_fdom !mem_filter //=.
             move => [] ain [m2o] tra xeq.
             split. smt(get_setE).
-            have->: oget GAKE_mod.GAKEb_nodhs.s_smap{2}.[x] = rem_sid_s (oget GAKEb_st.s_smap{1}.[a]). smt().
+            have->: oget UAKE_mod.O_RPK.s_smap{2}.[x] = rem_sid_s (oget UAKE_name_st.s_smap{1}.[a]). smt().
             have : (Pending_mod st{2} pk_e{2} ir{2}) = rem_sid_c (Pending st{1} pk_e{1} ir{1}). smt().
             rewrite /rem_sid_c //=.
             move => [#] steq pteq ireq.
@@ -2821,13 +2816,13 @@ case : (!(st1r \/ st2r)) => />. smt().
           have : st{1}.`2 = x.`1. smt(get_setE mem_set in_fsetU1 pow_bij).
           move => x1eq.
           split. split.
-          + have : pk_e{1}.`1 \in Name_Red.O_GAKE.sid_pk{2}. smt().
+          + have : pk_e{1}.`1 \in Name_Red.O_UAKE_RN.sid_pk{2}. smt().
           + smt(get_setE mem_set).
           + have v := inv2 pk_e{1}.`1 x.`2 st{1}.`2 pk_e{1}.`2 m2o.
             rewrite v; smt().
           smt(get_setE mem_set in_fsetU1 pow_bij).
-        have<-: (card (get_tested_origins_c (pk_e{1}, None) GAKEb_st.s_smap{1}) = card (get_tested_origins_c (pk_e{2}, None) GAKE_mod.GAKEb_nodhs.s_smap{2})).
-        + rewrite -(inj_fcard_image_pw (fun (bj : s_id * int) => (oget Name_Red.O_GAKE.sid_pk{2}.[bj.`1], bj.`2))).
+        have<-: (card (get_tested_origins_c (pk_e{1}, None) UAKE_name_st.s_smap{1}) = card (get_tested_origins_c (pk_e{2}, None) UAKE_mod.O_RPK.s_smap{2})).
+        + rewrite -(inj_fcard_image_pw (fun (bj : s_id * int) => (oget Name_Red.O_UAKE_RN.sid_pk{2}.[bj.`1], bj.`2))).
           + move => x y.
             rewrite !mem_fdom !mem_filter //=.
             smt(get_setE mem_set in_fsetU1 pow_bij).
@@ -2841,7 +2836,7 @@ case : (!(st1r \/ st2r)) => />. smt().
             rewrite !mem_fdom !mem_filter //=.
             move => [] ain [] [m2o] tra ant xeq.
             split. smt(get_setE).
-            have->: oget GAKE_mod.GAKEb_nodhs.s_smap{2}.[x] = rem_sid_s (oget GAKEb_st.s_smap{1}.[a]). smt().
+            have->: oget UAKE_mod.O_RPK.s_smap{2}.[x] = rem_sid_s (oget UAKE_name_st.s_smap{1}.[a]). smt().
             have : (Pending_mod st{2} pk_e{2} ir{2}) = rem_sid_c (Pending st{1} pk_e{1} ir{1}). smt().
             rewrite /rem_sid_c //=.
             move => [#] steq pteq ireq.
@@ -2860,7 +2855,7 @@ case : (!(st1r \/ st2r)) => />. smt().
           have : st{1}.`2 = x.`1. smt(get_setE mem_set in_fsetU1 pow_bij).
           move => x1eq.
           split. split.
-          + have : pk_e{1}.`1 \in Name_Red.O_GAKE.sid_pk{2}. smt().
+          + have : pk_e{1}.`1 \in Name_Red.O_UAKE_RN.sid_pk{2}. smt().
           + smt(get_setE mem_set).
           + have v := inv2 pk_e{1}.`1 x.`2 st{1}.`2 pk_e{1}.`2 m2o.
             rewrite v; smt().
@@ -2872,9 +2867,9 @@ case : (!(st1r \/ st2r)) => />. smt().
       if => //.
       + auto => /> &1 &2 25? inv inv2 *. 
         rewrite /tested_origins_c.
-        have<-: (card (get_origins_c t{1} GAKEb_st.s_smap{1}) = card (get_origins_c t{2} GAKE_mod.GAKEb_nodhs.s_smap{2})).
+        have<-: (card (get_origins_c t{1} UAKE_name_st.s_smap{1}) = card (get_origins_c t{2} UAKE_mod.O_RPK.s_smap{2})).
         + rewrite /get_origins_c.
-          rewrite -(inj_fcard_image_pw (fun (bj : s_id * int) => (oget Name_Red.O_GAKE.sid_pk{2}.[bj.`1], bj.`2))).
+          rewrite -(inj_fcard_image_pw (fun (bj : s_id * int) => (oget Name_Red.O_UAKE_RN.sid_pk{2}.[bj.`1], bj.`2))).
           + move => x y.
             rewrite !mem_fdom !mem_filter //=.
             smt(get_setE mem_set in_fsetU1 pow_bij).
@@ -2888,7 +2883,7 @@ case : (!(st1r \/ st2r)) => />. smt().
             rewrite !mem_fdom !mem_filter //=.
             move => [] ain [m2o] tra xeq.
             split; 1: smt(get_setE mem_set).
-            have->: oget GAKE_mod.GAKEb_nodhs.s_smap{2}.[x] = rem_sid_s (oget GAKEb_st.s_smap{1}.[a]) by smt().
+            have->: oget UAKE_mod.O_RPK.s_smap{2}.[x] = rem_sid_s (oget UAKE_name_st.s_smap{1}.[a]) by smt().
             have : (Accepted_mod st{2} t{2} k{2} ir{2}) = rem_sid_c (Accepted st{1} t{1} k{1} ir{1}) by smt().
             rewrite /rem_sid_c //=.
             move => [#] steq teq keq ireq.
@@ -2906,14 +2901,14 @@ case : (!(st1r \/ st2r)) => />. smt().
           have : st{1}.`2 = x.`1; 1: smt(get_setE mem_set in_fsetU1 pow_bij).
           move => x1eq.
           split. split.
-          + have : t{1}.`1.`1 \in Name_Red.O_GAKE.sid_pk{2}. smt().
+          + have : t{1}.`1.`1 \in Name_Red.O_UAKE_RN.sid_pk{2}. smt().
           + smt(get_setE mem_set).
           + have v := inv2 t{1}.`1.`1 x.`2 st{1}.`2 t{1}.`1.`2 m2o.
             rewrite v; smt().
           smt(get_setE mem_set in_fsetU1 pow_bij).
-        have<-: (card (get_tested_origins_c t{1} GAKEb_st.s_smap{1}) = card (get_tested_origins_c t{2} GAKE_mod.GAKEb_nodhs.s_smap{2})).
+        have<-: (card (get_tested_origins_c t{1} UAKE_name_st.s_smap{1}) = card (get_tested_origins_c t{2} UAKE_mod.O_RPK.s_smap{2})).
         + rewrite /get_tested_origins_c.
-          rewrite -(inj_fcard_image_pw (fun (bj : s_id * int) => (oget Name_Red.O_GAKE.sid_pk{2}.[bj.`1], bj.`2))).
+          rewrite -(inj_fcard_image_pw (fun (bj : s_id * int) => (oget Name_Red.O_UAKE_RN.sid_pk{2}.[bj.`1], bj.`2))).
           + move => x y.
             rewrite !mem_fdom !mem_filter //=.
             smt(get_setE mem_set in_fsetU1 pow_bij).
@@ -2927,7 +2922,7 @@ case : (!(st1r \/ st2r)) => />. smt().
             rewrite !mem_fdom !mem_filter //=.
             move => [] ain [] [m2o] tra ant xeq.
             split; 1: smt(get_setE mem_set).
-            have->: oget GAKE_mod.GAKEb_nodhs.s_smap{2}.[x] = rem_sid_s (oget GAKEb_st.s_smap{1}.[a]). smt().
+            have->: oget UAKE_mod.O_RPK.s_smap{2}.[x] = rem_sid_s (oget UAKE_name_st.s_smap{1}.[a]). smt().
             have : (Accepted_mod st{2} t{2} k{2} ir{2}) = rem_sid_c (Accepted st{1} t{1} k{1} ir{1}). smt().
             rewrite /rem_sid_c //=.
             move => [#] steq teq keq ireq.
@@ -2944,7 +2939,7 @@ case : (!(st1r \/ st2r)) => />. smt().
           exists (t{1}.`1.`1, x.`2).
           rewrite mem_fdom mem_filter //=.
           split. split.
-          + have : t{1}.`1.`1 \in Name_Red.O_GAKE.sid_pk{2}. smt().
+          + have : t{1}.`1.`1 \in Name_Red.O_UAKE_RN.sid_pk{2}. smt().
           + smt(get_setE mem_set).
           + have v := inv2 t{1}.`1.`1 x.`2 st{1}.`2 t{1}.`1.`2 m2o.
             rewrite v; smt().
@@ -2974,16 +2969,16 @@ case : (!(st1r \/ st2r)) => />. smt().
       + auto => /> &1 &2 15? inv ? inv2 *.
         rewrite /untested_partner_s.
         rewrite /get_partners_s.
-        have-> : (fdom (filter (fun (_ : int) (val : GAKEc.pr_st_client GAKEc.instance_state) => get_trace val 
-                   = Some t{1}) GAKEb_st.c_smap{1})) = (fdom (filter (fun (_ : int) (val : GAKE_mod.pr_st_client GAKE_mod.instance_state) 
-                 => get_trace val = Some t{2}) GAKE_mod.GAKEb_nodhs.c_smap{2})).
+        have-> : (fdom (filter (fun (_ : int) (val : UAKEc.c_state UAKEc.instance_state) => get_trace val 
+                   = Some t{1}) UAKE_name_st.c_smap{1})) = (fdom (filter (fun (_ : int) (val : UAKE_mod.c_state UAKE_mod.instance_state) 
+                 => get_trace val = Some t{2}) UAKE_mod.O_RPK.c_smap{2})).
         + rewrite fsetP.
           move => x.
           rewrite !mem_fdom !mem_filter //=.
           split. 
           + move => [] xin trx.
             split; 1: smt(get_setE mem_set in_fsetU1 pow_bij).
-            have->: oget GAKE_mod.GAKEb_nodhs.c_smap{2}.[x] = rem_sid_c (oget GAKEb_st.c_smap{1}.[x]) by smt().
+            have->: oget UAKE_mod.O_RPK.c_smap{2}.[x] = rem_sid_c (oget UAKE_name_st.c_smap{1}.[x]) by smt().
             have : (Accepted_mod st{2} t{2} k{2} ir{2}) = rem_sid_s (Accepted st{1} t{1} k{1} ir{1}) by smt().
             rewrite /rem_sid_s //=.
             move => [#] steq teq keq ireq.
@@ -2999,7 +2994,7 @@ case : (!(st1r \/ st2r)) => />. smt().
           move => [#] steq teq keq ireq.
           rewrite teq.
           move => [] xin.
-          have->: oget GAKE_mod.GAKEb_nodhs.c_smap{2}.[x] = rem_sid_c (oget GAKEb_st.c_smap{1}.[x]) by smt().
+          have->: oget UAKE_mod.O_RPK.c_smap{2}.[x] = rem_sid_c (oget UAKE_name_st.c_smap{1}.[x]) by smt().
           move => trx.
           have v := inv2 x (g ^ st{1}.`2) b{2} t{1}.`1.`2 t{1}.`2.
           rewrite v; 1,3,4: smt().
@@ -3007,16 +3002,16 @@ case : (!(st1r \/ st2r)) => />. smt().
             smt().
           smt(get_setE mem_set in_fsetU1 pow_bij).          
         rewrite /get_untested_partners_s.
-        have->: (fdom (filter (fun (_ : int) (val : GAKEc.pr_st_client GAKEc.instance_state) => get_trace val = Some t{1} /\ get_ir_test val = false) 
-                   GAKEb_st.c_smap{1})) = (fdom (filter (fun (_ : int) (val : GAKE_mod.pr_st_client GAKE_mod.instance_state) => get_trace val 
-                 = Some t{2} /\ get_ir_test val = false) GAKE_mod.GAKEb_nodhs.c_smap{2})).
+        have->: (fdom (filter (fun (_ : int) (val : UAKEc.c_state UAKEc.instance_state) => get_trace val = Some t{1} /\ get_ir_test val = false) 
+                   UAKE_name_st.c_smap{1})) = (fdom (filter (fun (_ : int) (val : UAKE_mod.c_state UAKE_mod.instance_state) => get_trace val 
+                 = Some t{2} /\ get_ir_test val = false) UAKE_mod.O_RPK.c_smap{2})).
         + rewrite fsetP.
           move => x.
           rewrite !mem_fdom !mem_filter //=.
           split. 
           + move => [] xin trx.
             split; 1: smt(get_setE mem_set in_fsetU1 pow_bij).
-            have->: oget GAKE_mod.GAKEb_nodhs.c_smap{2}.[x] = rem_sid_c (oget GAKEb_st.c_smap{1}.[x]) by smt().
+            have->: oget UAKE_mod.O_RPK.c_smap{2}.[x] = rem_sid_c (oget UAKE_name_st.c_smap{1}.[x]) by smt().
             have : (Accepted_mod st{2} t{2} k{2} ir{2}) = rem_sid_s (Accepted st{1} t{1} k{1} ir{1}) by smt().
             rewrite /rem_sid_s //=.
             move => [#] steq teq keq ireq.
@@ -3033,7 +3028,7 @@ case : (!(st1r \/ st2r)) => />. smt().
           move => [#] steq teq keq ireq.
           rewrite teq.
           move => [] xin.
-          have->: oget GAKE_mod.GAKEb_nodhs.c_smap{2}.[x] = rem_sid_c (oget GAKEb_st.c_smap{1}.[x]) by smt().
+          have->: oget UAKE_mod.O_RPK.c_smap{2}.[x] = rem_sid_c (oget UAKE_name_st.c_smap{1}.[x]) by smt().
           move => trx.
           have v := inv2 x (g ^ st{1}.`2) b{2} t{1}.`1.`2 t{1}.`2.
           rewrite v; smt().
@@ -3063,9 +3058,9 @@ case : (!(st1r \/ st2r)) => />. smt().
         if => //.
         + auto => /> &1 &2 25? inv inv2 *. 
           rewrite /fresh_partner_c.
-          have<-: (card (get_partners_c t'{1} GAKEb_st.s_smap{1}) = card (get_partners_c t'{2} GAKE_mod.GAKEb_nodhs.s_smap{2})).
+          have<-: (card (get_partners_c t'{1} UAKE_name_st.s_smap{1}) = card (get_partners_c t'{2} UAKE_mod.O_RPK.s_smap{2})).
           + rewrite /get_partners_c. 
-            rewrite -(inj_fcard_image_pw (fun (bj : s_id * int) => (oget Name_Red.O_GAKE.sid_pk{2}.[bj.`1], bj.`2))).
+            rewrite -(inj_fcard_image_pw (fun (bj : s_id * int) => (oget Name_Red.O_UAKE_RN.sid_pk{2}.[bj.`1], bj.`2))).
             + move => x y.
               rewrite !mem_fdom !mem_filter //=.
               smt(get_setE mem_set in_fsetU1 pow_bij).
@@ -3079,7 +3074,7 @@ case : (!(st1r \/ st2r)) => />. smt().
               rewrite !mem_fdom !mem_filter //=.
               move => [] ain tra xeq.
               split; 1: smt(get_setE).
-              have->: oget GAKE_mod.GAKEb_nodhs.s_smap{2}.[x] = rem_sid_s (oget GAKEb_st.s_smap{1}.[a]) by smt().
+              have->: oget UAKE_mod.O_RPK.s_smap{2}.[x] = rem_sid_s (oget UAKE_name_st.s_smap{1}.[a]) by smt().
               have : (Accepted_mod st'{2} t'{2} k'{2} ir'{2}) = rem_sid_c (Accepted st'{1} t'{1} k'{1} ir'{1})  by smt().
               rewrite /rem_sid_c //=.
               move => [#] steq teq keq ireq.
@@ -3096,14 +3091,14 @@ case : (!(st1r \/ st2r)) => />. smt().
             have : st'{1}.`2 = x.`1 by smt(get_setE mem_set in_fsetU1 pow_bij).
             move => x1eq.
             split. split.
-            + have : t'{1}.`1.`1 \in Name_Red.O_GAKE.sid_pk{2} by smt().
+            + have : t'{1}.`1.`1 \in Name_Red.O_UAKE_RN.sid_pk{2} by smt().
               smt(get_setE mem_set).
             + have v := inv2 t'{1}.`1.`1 x.`2 st'{1}.`2 t'{1}.`1.`2 t'{1}.`2.
               rewrite v; smt().
             smt(get_setE mem_set in_fsetU1 pow_bij).          
-          have<-: (card (get_fresh_partners_c t'{1} GAKEb_st.s_smap{1} GAKEb_st.servers{1}) 
-                    = card (get_fresh_partners_c t'{2} GAKE_mod.GAKEb_nodhs.s_smap{2} GAKE_mod.GAKEb_nodhs.servers{2})).
-          + rewrite -(inj_fcard_image_pw (fun (bj : s_id * int) => (oget Name_Red.O_GAKE.sid_pk{2}.[bj.`1], bj.`2))).
+          have<-: (card (get_fresh_partners_c t'{1} UAKE_name_st.s_smap{1} UAKE_name_st.servers{1}) 
+                    = card (get_fresh_partners_c t'{2} UAKE_mod.O_RPK.s_smap{2} UAKE_mod.O_RPK.servers{2})).
+          + rewrite -(inj_fcard_image_pw (fun (bj : s_id * int) => (oget Name_Red.O_UAKE_RN.sid_pk{2}.[bj.`1], bj.`2))).
             + move => x y.
               rewrite !mem_fdom !mem_filter //=.
               smt(get_setE mem_set in_fsetU1 pow_bij).
@@ -3117,7 +3112,7 @@ case : (!(st1r \/ st2r)) => />. smt().
               rewrite !mem_fdom !mem_filter //=.
               move => [#] ain tra ant ansr antb xeq.
               split; 1: smt(get_setE).
-              have->: oget GAKE_mod.GAKEb_nodhs.s_smap{2}.[x] = rem_sid_s (oget GAKEb_st.s_smap{1}.[a]) by smt().
+              have->: oget UAKE_mod.O_RPK.s_smap{2}.[x] = rem_sid_s (oget UAKE_name_st.s_smap{1}.[a]) by smt().
               have : (Accepted_mod st'{2} t'{2} k'{2} ir'{2}) = rem_sid_c (Accepted st'{1} t'{1} k'{1} ir'{1}) by smt().
               rewrite /rem_sid_c //=.
               move => [#] steq teq keq ireq.
@@ -3135,7 +3130,7 @@ case : (!(st1r \/ st2r)) => />. smt().
             have : st'{1}.`2 = x.`1 by smt(get_setE mem_set in_fsetU1 pow_bij).
             move => x1eq.
             split. split.
-            + have : t'{1}.`1.`1 \in Name_Red.O_GAKE.sid_pk{2} by smt().
+            + have : t'{1}.`1.`1 \in Name_Red.O_UAKE_RN.sid_pk{2} by smt().
               smt(get_setE mem_set).
             + have v := inv2 t'{1}.`1.`1 x.`2 st'{1}.`2 t'{1}.`1.`2 t'{1}.`2.
               clear inv inv2.
@@ -3173,15 +3168,15 @@ case : (!(st1r \/ st2r)) => />. smt().
         + auto => /> &1 &2 15? inv ? inv2 *.
           rewrite /fresh_partner_s.
           rewrite /get_origins_s.
-          have-> : (fdom (filter (fun (_ : int) (val : GAKEc.pr_st_client GAKEc.instance_state) => exists (m2o : (pkey * tag) option),
-                      get_trace val = Some (t'{1}.`1, m2o)) GAKEb_st.c_smap{1})) = fdom (filter (fun (_ : int) (val : GAKE_mod.pr_st_client GAKE_mod.instance_state) =>
-                    exists (m2o : (pkey * tag) option), get_trace val = Some (t'{2}.`1, m2o)) GAKE_mod.GAKEb_nodhs.c_smap{2}).
+          have-> : (fdom (filter (fun (_ : int) (val : UAKEc.c_state UAKEc.instance_state) => exists (m2o : (pkey * tag) option),
+                      get_trace val = Some (t'{1}.`1, m2o)) UAKE_name_st.c_smap{1})) = fdom (filter (fun (_ : int) (val : UAKE_mod.c_state UAKE_mod.instance_state) =>
+                    exists (m2o : (pkey * tag) option), get_trace val = Some (t'{2}.`1, m2o)) UAKE_mod.O_RPK.c_smap{2}).
           + rewrite fsetP.
             move => x.
             rewrite !mem_fdom !mem_filter //=.
             split. 
             + move => [] xin.
-              have->: oget GAKE_mod.GAKEb_nodhs.c_smap{2}.[x] = rem_sid_c (oget GAKEb_st.c_smap{1}.[x]) by smt().
+              have->: oget UAKE_mod.O_RPK.c_smap{2}.[x] = rem_sid_c (oget UAKE_name_st.c_smap{1}.[x]) by smt().
               have : (Accepted_mod st'{2} t'{2} k'{2} ir'{2}) = rem_sid_s (Accepted st'{1} t'{1} k'{1} ir'{1}) by smt().
               rewrite /rem_sid_s //=.
               move => [#] steq teq keq ireq.
@@ -3196,22 +3191,22 @@ case : (!(st1r \/ st2r)) => />. smt().
             move => [#] steq teq keq ireq.
             rewrite teq.
             move => [] xin.
-            have->: oget GAKE_mod.GAKEb_nodhs.c_smap{2}.[x] = rem_sid_c (oget GAKEb_st.c_smap{1}.[x]) by smt().
+            have->: oget UAKE_mod.O_RPK.c_smap{2}.[x] = rem_sid_c (oget UAKE_name_st.c_smap{1}.[x]) by smt().
             move => [m2o] trx.
             split; 1: smt(get_setE mem_set in_fsetU1 pow_bij).
             have v := inv2 x (g ^ st'{1}.`2) b{2} t'{1}.`1.`2 m2o.
             rewrite v; smt().
           rewrite /get_fresh_partners_s.
-          have->: (fdom (filter (fun (_ : int) (val : GAKEc.pr_st_client GAKEc.instance_state) => (exists (m2o : (pkey * tag) option), get_trace val 
-                     = Some (t'{1}.`1, m2o)) /\ get_ir_test val = false /\  get_ir_sess val = false /\ get_ir_eph val = false) GAKEb_st.c_smap{1})) 
-                   = (fdom (filter (fun (_ : int) (val : GAKE_mod.pr_st_client GAKE_mod.instance_state) => (exists (m2o : (pkey * tag) option), get_trace val 
-                     = Some (t'{2}.`1, m2o)) /\ get_ir_test val = false /\  get_ir_sess val = false /\ get_ir_eph val = false) GAKE_mod.GAKEb_nodhs.c_smap{2})).
+          have->: (fdom (filter (fun (_ : int) (val : UAKEc.c_state UAKEc.instance_state) => (exists (m2o : (pkey * tag) option), get_trace val 
+                     = Some (t'{1}.`1, m2o)) /\ get_ir_test val = false /\  get_ir_sess val = false /\ get_ir_eph val = false) UAKE_name_st.c_smap{1})) 
+                   = (fdom (filter (fun (_ : int) (val : UAKE_mod.c_state UAKE_mod.instance_state) => (exists (m2o : (pkey * tag) option), get_trace val 
+                     = Some (t'{2}.`1, m2o)) /\ get_ir_test val = false /\  get_ir_sess val = false /\ get_ir_eph val = false) UAKE_mod.O_RPK.c_smap{2})).
             rewrite fsetP.
             move => x.
             rewrite !mem_fdom !mem_filter //=.
             split. 
             + move => [] xin.
-              have->: oget GAKE_mod.GAKEb_nodhs.c_smap{2}.[x] = rem_sid_c (oget GAKEb_st.c_smap{1}.[x]) by smt().
+              have->: oget UAKE_mod.O_RPK.c_smap{2}.[x] = rem_sid_c (oget UAKE_name_st.c_smap{1}.[x]) by smt().
               have : (Accepted_mod st'{2} t'{2} k'{2} ir'{2}) = rem_sid_s (Accepted st'{1} t'{1} k'{1} ir'{1}) by smt().
               rewrite /rem_sid_s //=.
               move => [#] steq teq keq ireq.
@@ -3229,7 +3224,7 @@ case : (!(st1r \/ st2r)) => />. smt().
             move => [#] steq teq keq ireq.
             rewrite teq.
             move => [] xin.
-            have->: oget GAKE_mod.GAKEb_nodhs.c_smap{2}.[x] = rem_sid_c (oget GAKEb_st.c_smap{1}.[x]) by smt().
+            have->: oget UAKE_mod.O_RPK.c_smap{2}.[x] = rem_sid_c (oget UAKE_name_st.c_smap{1}.[x]) by smt().
             move => [] [m2o] trx xfresh.
             split; 1: smt(get_setE mem_set in_fsetU1 pow_bij).
             have v := inv2 x (g ^ st'{1}.`2) b{2} t'{1}.`1.`2 m2o.
@@ -3248,7 +3243,7 @@ case : (!(st1r \/ st2r)) => />. smt().
             rewrite !mem_fdom !mem_filter //=.
             split. 
             + move => [] xin.
-              have->: oget GAKE_mod.GAKEb_nodhs.c_smap{2}.[x] = rem_sid_c (oget GAKEb_st.c_smap{1}.[x]) by smt().
+              have->: oget UAKE_mod.O_RPK.c_smap{2}.[x] = rem_sid_c (oget UAKE_name_st.c_smap{1}.[x]) by smt().
               have : (Accepted_mod st'{2} t'{2} k'{2} ir'{2}) = rem_sid_s (Accepted st'{1} t'{1} k'{1} ir'{1}) by smt().
               rewrite /rem_sid_s //=.
               move => [#] steq teq keq ireq.
@@ -3265,7 +3260,7 @@ case : (!(st1r \/ st2r)) => />. smt().
             move => [#] steq teq keq ireq.
             rewrite teq.
             move => [] xin.
-            have->: oget GAKE_mod.GAKEb_nodhs.c_smap{2}.[x] = rem_sid_c (oget GAKEb_st.c_smap{1}.[x]) by smt().
+            have->: oget UAKE_mod.O_RPK.c_smap{2}.[x] = rem_sid_c (oget UAKE_name_st.c_smap{1}.[x]) by smt().
             move => [] [m2o] trx xfresh.
             split; 1: smt(get_setE mem_set in_fsetU1 pow_bij).
             have v := inv2 x (g ^ st'{1}.`2) b{2} t'{1}.`1.`2 m2o.
@@ -3282,7 +3277,7 @@ case : (!(st1r \/ st2r)) => />. smt().
           rewrite !mem_fdom !mem_filter //=.
           split. 
           + move => [] xin.
-            have->: oget GAKE_mod.GAKEb_nodhs.c_smap{2}.[x] = rem_sid_c (oget GAKEb_st.c_smap{1}.[x]) by smt().
+            have->: oget UAKE_mod.O_RPK.c_smap{2}.[x] = rem_sid_c (oget UAKE_name_st.c_smap{1}.[x]) by smt().
             have : (Accepted_mod st'{2} t'{2} k'{2} ir'{2}) = rem_sid_s (Accepted st'{1} t'{1} k'{1} ir'{1}) by smt().
             rewrite /rem_sid_s //=.
             move => [#] steq teq keq ireq.
@@ -3299,7 +3294,7 @@ case : (!(st1r \/ st2r)) => />. smt().
           move => [#] steq teq keq ireq.
           rewrite teq.
           move => [] xin.
-          have->: oget GAKE_mod.GAKEb_nodhs.c_smap{2}.[x] = rem_sid_c (oget GAKEb_st.c_smap{1}.[x]) by smt().
+          have->: oget UAKE_mod.O_RPK.c_smap{2}.[x] = rem_sid_c (oget UAKE_name_st.c_smap{1}.[x]) by smt().
           move => [] [m2o] trx xfresh.
           split; 1: smt(get_setE mem_set in_fsetU1 pow_bij).
           have v := inv2 x (g ^ st'{1}.`2) b{2} t'{1}.`1.`2 m2o.
@@ -3323,16 +3318,16 @@ case : (!(st1r \/ st2r)) => />. smt().
 qed.
 
 
-lemma name_to_pk bit &m: `| Pr[GAKEc.E_GAKE_nodhs(GAKEc.GAKEb_nodhs(NTOR_S, NTOR_C, GAKEc.HROc.RO), A_res).run(bit) @ &m : res]
-     - Pr[GAKE_mod.E_GAKE_nodhs(GAKE_mod.GAKEb_nodhs(NTOR_S_mod, NTOR_C_mod, GAKE_mod.HROc.RO), Name_Red(A_res)).run(bit) @ &m : res] | 
+lemma name_to_pk bit &m: `| Pr[UAKEc.E_UAKE_RN(UAKEc.O_RN(NTOR_S, NTOR_C, UAKEc.HROc.RO), A_res).run(bit) @ &m : res]
+     - Pr[UAKE_mod.E_UAKE(UAKE_mod.O_RPK(S, C, UAKE_mod.HROc.RO), Name_Red(A_res)).run(bit) @ &m : res] | 
                  <= ((q_is + q_m1 + q_m2) * (q_is + q_m1 + q_m2 - 1))%r / (2 * order)%r
                      + ((q_h + q_m1 + q_m2 + q_m3) * (q_h + q_m1 + q_m2 + q_m3 - 1))%r / (2 * order)%r.
 proof. 
 rewrite gake_st.
-apply (ler_trans (Pr[GAKEc.E_GAKE_nodhs(GAKEb_st(NTOR_S, NTOR_C, GAKEc.HROc.RO), A_res).run(bit) @ &m : (GAKEb_st.stop1 \/ GAKEb_st.stop2)])).
+apply (ler_trans (Pr[UAKEc.E_UAKE_RN(UAKE_name_st(NTOR_S, NTOR_C, UAKEc.HROc.RO), A_res).run(bit) @ &m : (UAKE_name_st.stop1 \/ UAKE_name_st.stop2)])).
 + apply gake_no_name.
-apply (ler_trans (Pr[GAKEc.E_GAKE_nodhs(GAKEb_st(NTOR_S, NTOR_C, GAKEc.HROc.RO), A_res).run(bit) @ &m : GAKEb_st.stop1] 
-      + Pr[GAKEc.E_GAKE_nodhs(GAKEb_st(NTOR_S, NTOR_C, GAKEc.HROc.RO), A_res).run(bit) @ &m : GAKEb_st.stop2])).
+apply (ler_trans (Pr[UAKEc.E_UAKE_RN(UAKE_name_st(NTOR_S, NTOR_C, UAKEc.HROc.RO), A_res).run(bit) @ &m : UAKE_name_st.stop1] 
+      + Pr[UAKEc.E_UAKE_RN(UAKE_name_st(NTOR_S, NTOR_C, UAKEc.HROc.RO), A_res).run(bit) @ &m : UAKE_name_st.stop2])).
 + apply sum_stop.
 smt(bound_stop1 bound_stop2).
 qed.
